use "x x_extra" instead of "x_base x"
_base was nonsensical anyways and this should be simpler for some stuff

DependentComputability/NewDecls.lean
@@ -17,7 +17,7 @@ protected def Nat.zero : new_type% @Nat.zero := ()
 protected def Nat.succ : new_type% @Nat.succ := fun _ _ => ()
 
 protected def Nat.rec.{u} : new_type% @Nat.rec.{u} :=
-  fun {_} _ {_} zero {_} succ {t_base} _ => t_base.rec zero fun _ ih => succ () ih
+  fun {_} _ {_} zero {_} succ {t} _ => t.rec zero fun _ ih => succ () ih
 
 protected def PUnit.{u} : new_type% @PUnit.{u} :=
   .mk (fun _ => PUnit.{u}) (TrivialEncoding _) (.trivialEncoding _)
@@ -26,14 +26,14 @@ protected def PUnit.unit.{u} : new_type% @PUnit.unit.{u} :=
   @_root_.PUnit.unit.{u}
 
 protected theorem propext : new_type% @propext := by
-  intro p_base p q_base q h_base h
+  intro p p_extra q q_extra h h_extra
   dsimp only
-  cases propext h_base
-  rcases p with ⟨pty, penc, pelim⟩
-  rcases q with ⟨qty, qenc, qelim⟩
+  cases propext h
+  rcases p_extra with ⟨pty, penc, pelim⟩
+  rcases q_extra with ⟨qty, qenc, qelim⟩
   cases pelim.eq
   cases qelim.eq
-  rcases h with ⟨hmp, hmpr⟩
+  rcases h_extra with ⟨hmp, hmpr⟩
   have : pty = qty := by
     ext h
     exact ⟨@hmp h, @hmpr h⟩
@@ -43,117 +43,117 @@ protected theorem propext : new_type% @propext := by
 set_option bootstrap.inductiveCheckResultingUniverse false in
 set_option genSizeOf false in
 set_option genInjectivity false in
-inductive Quot._base {α_base : Sort u} {α : new_type% α_base}
-    {r_base : α_base → α_base → Prop} (r : new_type% r_base) :
-    Quot r_base → Sort u where
-  | mk {a_base : α_base} (a : α.1 a_base) : _base r (Quot.mk r_base a_base)
+inductive Quot._base {α : Sort u} {α_extra : new_type% α}
+    {r : α → α → Prop} (r_extra : new_type% r) :
+    Quot r → Sort u where
+  | mk {a : α} (a_extra : α_extra.1 a) : _base r_extra (Quot.mk r a)
 
-inductive Quot._rel {α_base : Sort u} {α : new_type% α_base}
-    {r_base : α_base → α_base → Prop} (r : new_type% r_base) :
-    (q : Quot r_base) → Quot._base r q → Quot._base r q → Prop where
-  | mk {a_base : α_base} (a : α.1 a_base) {b_base : α_base} (b : α.1 b_base)
-    {h_base : r_base a_base b_base} (h : (r a b).1 h_base) :
-    _rel r (Quot.mk r_base b_base) (Quot.sound h_base ▸ .mk a) (.mk b)
+inductive Quot._rel {α : Sort u} {α_extra : new_type% α}
+    {r : α → α → Prop} (r_extra : new_type% r) :
+    (q : Quot r) → Quot._base r_extra q → Quot._base r_extra q → Prop where
+  | mk {a : α} (a_extra : α_extra.1 a) {b : α} (b_extra : α_extra.1 b)
+    {h : r a b} (h_extra : (r_extra a_extra b_extra).1 h) :
+    _rel r_extra (Quot.mk r b) (Quot.sound h ▸ .mk a_extra) (.mk b_extra)
 
-inductive Quot._encoding {α_base : Sort u} {α : new_type% α_base}
-    {r_base : α_base → α_base → Prop} (r : new_type% r_base) :
-    ⦃q_base : Quot r_base⦄ → (q : Quot (_rel r q_base)) → (n : ℕ) → Prop where
-  | mk {a_base : α_base} {a : α.1 a_base} {n : ℕ} (h : α.2 a n) :
-    @_encoding α_base α r_base r (Quot.mk r_base a_base) (Quot.mk _ (.mk a)) n
+inductive Quot._encoding {α : Sort u} {α_extra : new_type% α}
+    {r : α → α → Prop} (r_extra : new_type% r) :
+    ⦃q : Quot r⦄ → (q : Quot (_rel r_extra q)) → (n : ℕ) → Prop where
+  | mk {a : α} {a_extra : α_extra.1 a} {n : ℕ} (h : α_extra.2 a_extra n) :
+    @_encoding α α_extra r r_extra (Quot.mk r a) (Quot.mk _ (.mk a_extra)) n
 
-protected def Quot.{u} : new_type% @Quot.{u} := fun α_base α r_base r =>
-  .mk (fun q => Quot (Quot._rel r q)) (Quot._encoding r) <| by
-    intro hprop a_base a n
+protected def Quot.{u} : new_type% @Quot.{u} := fun α α_extra r r_extra =>
+  .mk (fun q => Quot (Quot._rel r_extra q)) (Quot._encoding r_extra) <| by
+    intro hprop a a_extra n
     simp only [trivialEncoding_iff]
     constructor
     · rintro ⟨h⟩
-      simpa using (α.3 hprop _ _).mp h
+      simpa using (α_extra.3 hprop _ _).mp h
     · rintro rfl
-      rcases a with ⟨@⟨a_base, a'⟩⟩
+      rcases a_extra with ⟨@⟨a, a'⟩⟩
       constructor
-      exact (α.3 hprop _ _).mpr .zero
+      exact (α_extra.3 hprop _ _).mpr .zero
 
 protected def Quot.mk.{u} : new_type% @Quot.mk.{u} := fun _ _ _ _ _ a =>
   _root_.Quot.mk _ (.mk a)
 
 protected theorem Quot.ind.{u} : new_type% @Quot.ind.{u} := by
-  intro α_base α r_base r motive_base motive mk_base mk t_base t
-  rcases t with ⟨@⟨t_base, t⟩⟩
+  intro α α_extra r r_extra motive motive mk mk t t
+  rcases t with ⟨@⟨t, t⟩⟩
   apply mk
 
 protected def Quot.lift.{u, v} : new_type% @Quot.lift.{u, v} :=
-  fun α_base α r_base r β_base β f_base f h_base h q_base q =>
-    _root_.Quot.lift (fun x : _base r q_base =>
-      haveI : _root_.Quot.lift f_base h_base q_base = f_base x.1 := by
-        rcases x with @⟨a_base, a⟩
+  fun α α_extra r r_extra β β_extra f f_extra h h_extra q q_extra =>
+    _root_.Quot.lift (fun x : _base r_extra q =>
+      haveI : _root_.Quot.lift f h q = f x.1 := by
+        rcases x with @⟨a, a⟩
         rfl
-      this ▸ f x.2) ?_ q
+      this ▸ f_extra x.2) ?_ q_extra
 where finally
-  rintro _ _ @⟨a_base, a, b_base, b, hab_base, hab⟩
+  rintro _ _ @⟨a, a_extra, b, b_extra, hab, hab_extra⟩
   dsimp only
-  rw! (castMode := .all) [← Quot.sound hab_base]
-  change h_base a_base b_base hab_base ▸ f a = f b
-  refine (h a b hab).rec ?_
+  rw! (castMode := .all) [← Quot.sound hab]
+  change h a b hab ▸ f_extra a_extra = f_extra b_extra
+  refine (h_extra a_extra b_extra hab_extra).rec ?_
   rfl
 
 protected theorem Quot.sound.{u} : new_type% @Quot.sound.{u} := by
-  intro α_base α r_base r a_base a b_base b h_base h
+  intro α α_extra r r_extra a a_extra b b_extra h h_extra
   dsimp only
-  have sound_base := _root_.Quot.sound h_base
-  have sound := _root_.Quot.sound (Quot._rel.mk a b h)
+  have sound := _root_.Quot.sound h
+  have sound_extra := _root_.Quot.sound (Quot._rel.mk a_extra b_extra h_extra)
   simp only [Quot.mk]
-  rw! [← sound, ← sound_base]
+  rw! [← sound_extra, ← sound]
   constructor
 
 theorem subsingletonExtra_of_subsingleton
-    {α_base : Sort u} (α : New.Sort.1 α_base)
-    {h_base : _root_.Subsingleton α_base} (h : new_type% h_base) :
-    SubsingletonExtra α := by
+    {α : Sort u} (α_extra : new_type% α)
+    {h : _root_.Subsingleton α} (h_extra : new_type% h) :
+    SubsingletonExtra α_extra := by
   constructor
   intro x
   constructor
   intro a b
-  cases h.1 a b
+  cases h_extra.1 a b
   rfl
 
-instance {α_base : Sort u} (α : New.Sort.1 α_base) : SubsingletonExtra (new% Squash α_base) :=
-  subsingletonExtra_of_subsingleton _ (new% @instSubsingletonSquash α_base)
+instance {α : Sort u} (α_extra : new_type% α) : SubsingletonExtra (new% Squash α) :=
+  subsingletonExtra_of_subsingleton _ (new% @instSubsingletonSquash α)
 
 protected noncomputable def uniqueChoice.{u} : new_type% @uniqueChoice.{u} :=
-  fun α_base α h_base h =>
-    haveI : _root_.Nonempty ((a : α_base) ×' α.1 a) := by
-      obtain @⟨a_base, a⟩ := h
-      exact ⟨a_base, a⟩
+  fun α α_extra h h_extra =>
+    haveI : _root_.Nonempty ((a : α) ×' α_extra.1 a) := by
+      obtain @⟨a, a_extra⟩ := h_extra
+      exact ⟨a, a_extra⟩
     (uniqueChoice this).liftOn (fun x =>
-        haveI : uniqueChoice h_base = _root_.Squash.mk x.1 := Subsingleton.allEq ..
+        haveI : uniqueChoice h = _root_.Squash.mk x.1 := Subsingleton.allEq ..
         this ▸ Squash.mk _ x.2) (by intros; apply Subsingleton.allEq)
 
 end New
 
-instance {α_base : Sort u} (α : new_type% α_base) [SubsingletonExtra α]
-    {a_base : α_base} (a : α.1 a_base)
-    {b_base : α_base} (b : α.1 b_base) :
-    InhabitedExtra (New.Eq α a b) where
+instance {α : Sort u} (α_extra : new_type% α) [SubsingletonExtra α_extra]
+    {a : α} (a_extra : new_type% a)
+    {b : α} (b_extra : new_type% b) :
+    InhabitedExtra (new% a = b) where
   default := by
     rintro rfl
-    cases (SubsingletonExtra.subsingleton a_base).allEq a b
+    cases (SubsingletonExtra.subsingleton a).allEq a_extra b_extra
     constructor
 
 instance : FullyRepresentable New.Nat where
   default _ := ()
   subsingleton _ := inferInstanceAs (Subsingleton Unit)
-  isRepresentable {x_base} _ := ⟨x_base, rfl⟩
+  isRepresentable {x} _ := ⟨x, rfl⟩
 
 def uniqueNatVal (n : Nat) : new_type% n := ()
 
-inductive New.Subtype._induct {α_base : Sort u} {α : new_type% α_base}
-    {p_base : α_base → Prop} (p : new_type% p_base) (t : Subtype p_base) where
-  | mk (val : α.1 t.1) (property : (p val).1 t.2)
+inductive New.Subtype._induct {α : Sort u} {α_extra : new_type% α}
+    {p : α → Prop} (p_extra : new_type% p) (t : Subtype p) where
+  | mk (val : α_extra.1 t.1) (property : (p_extra val).1 t.2)
 
-inductive New.Subtype._encoding {α_base : Sort u} {α : new_type% α_base}
-    {p_base : α_base → Prop} (p : new_type% p_base)
-    ⦃t_base : Subtype p_base⦄ (t : _induct p t_base) (n : ℕ) : Prop where
-  | mk (val_enc : α.2 t.1 n)
+inductive New.Subtype._encoding {α : Sort u} {α_extra : new_type% α}
+    {p : α → Prop} (p_extra : new_type% p)
+    ⦃t : Subtype p⦄ (t_extra : _induct p_extra t) (n : ℕ) : Prop where
+  | mk (val_enc : α_extra.2 t_extra.1 n)
 
 def New.Subtype : new_type% @Subtype.{u} := fun _ _ _ p =>
   .mk (Subtype._induct p) (Subtype._encoding p) (.univElim _)
@@ -165,58 +165,59 @@ def New.Subtype.rec.{v, u} : new_type% @Subtype.rec.{v, u} :=
   fun _ _ _ _ _ _ _ intro _ t => intro t.1 t.2
 
 @[simp]
-theorem encoding_subtype_def {α_base : Sort u} {α : new_type% α_base}
-    {p_base : α_base → Prop} {p : new_type% p_base}
-    {t_base : Subtype p_base} {t : new_type% t_base} {n : ℕ} :
-    (new% Subtype p_base).2 t n ↔ α.2 t.1 n := by
+theorem encoding_subtype_def {α : Sort u} {α_extra : new_type% α}
+    {p : α → Prop} {p_extra : new_type% p}
+    {t : Subtype p} {t_extra : new_type% t} {n : ℕ} :
+    (new% Subtype p).2 t_extra n ↔ α_extra.2 t_extra.1 n := by
   constructor
   · rintro ⟨h⟩
     exact h
   · intro h
     exact ⟨h⟩
 
-inductive New.List._induct {α_base : Type u} (α_extra : α_base → Type u) :
-    List α_base → Type u where
+inductive New.List._induct {α : Type u} (α_extra : α → Type u) :
+    List α → Type u where
   | nil : _induct α_extra []
-  | cons {head_base : α_base} (head : α_extra head_base)
-    {tail_base : List α_base} (tail : _induct α_extra tail_base) :
-    _induct α_extra (head_base :: tail_base)
+  | cons {head : α} (head_extra : α_extra head)
+    {tail : List α} (tail_extra : _induct α_extra tail) :
+    _induct α_extra (head :: tail)
 
-inductive New.List._encoding {α_base : Type u}
-    (α_extra : α_base → Type u) (α_enc : ⦃t_base : α_base⦄ → α_extra t_base → ℕ → Prop) :
-    ⦃l_base : List α_base⦄ → _induct α_extra l_base → ℕ → Prop where
+inductive New.List._encoding {α : Type u}
+    (α_extra : α → Type u) (α_enc : ⦃t : α⦄ → α_extra t → ℕ → Prop) :
+    ⦃l : List α⦄ → _induct α_extra l → ℕ → Prop where
   | nil : _encoding α_extra α_enc .nil (Nat.pair 0 1)
-  | cons {head_base : α_base} {head : α_extra head_base}
-    {head_n : ℕ} (head_enc : α_enc head head_n)
-    {tail_base : List α_base} {tail : _induct α_extra tail_base}
-    {tail_n : ℕ} (tail_enc : _encoding α_extra α_enc tail tail_n) :
-    _encoding α_extra α_enc (.cons head tail) (Nat.pair (Nat.pair head_n tail_n) 2)
+  | cons {head : α} {head_extra : α_extra head}
+    {head_n : ℕ} (head_enc : α_enc head_extra head_n)
+    {tail : List α} {tail_extra : _induct α_extra tail}
+    {tail_n : ℕ} (tail_enc : _encoding α_extra α_enc tail_extra tail_n) :
+    _encoding α_extra α_enc (.cons head_extra tail_extra)
+      (Nat.pair (Nat.pair head_n tail_n) 2)
 
 def New.List : new_type% @List.{u} :=
-  fun _ α => .mk (New.List._induct α.1) (New.List._encoding α.1 α.2)
+  fun _ α_extra => .mk (New.List._induct α_extra.1) (New.List._encoding α_extra.1 α_extra.2)
     (IsPropEncodingTrivial.univElim.{u + 1} _)
 
 def New.List.nil : new_type% @List.nil.{u} :=
-  fun _ α => @New.List._induct.nil _ α.1
+  fun _ α_extra => @New.List._induct.nil _ α_extra.1
 
 def New.List.cons : new_type% @List.cons.{u} :=
-  fun _ α => @New.List._induct.cons _ α.1
+  fun _ α_extra => @New.List._induct.cons _ α_extra.1
 
 noncomputable def New.List.rec.{u, v} : new_type% @List.rec.{u, v} :=
   fun _ _ _ _ _ nil _ cons _ t => t.rec nil (fun _ _ _ ih => cons _ _ ih)
 
 set_option inductive.autoPromoteIndices false in
-inductive New.Array._induct {α_base : Type u} (α_extra : α_base → Type u)
-    (t : Array α_base) : Type u where
+inductive New.Array._induct {α : Type u} (α_extra : α → Type u)
+    (t : Array α) : Type u where
   | mk (toList : New.List._induct α_extra t.1) : _induct α_extra t
 
-inductive New.Array._encoding {α_base : Type u}
-    (α_extra : α_base → Type u) (α_enc : ⦃t_base : α_base⦄ → α_extra t_base → ℕ → Prop)
-    ⦃l_base : Array α_base⦄ (l : _induct α_extra l_base) (n : ℕ) : Prop where
+inductive New.Array._encoding {α : Type u}
+    (α_extra : α → Type u) (α_enc : ⦃t : α⦄ → α_extra t → ℕ → Prop)
+    ⦃l : Array α⦄ (l : _induct α_extra l) (n : ℕ) : Prop where
   | mk (toList : New.List._encoding α_extra α_enc l.1 n)
 
 def New.Array : new_type% @Array.{u} :=
-  fun _ α => .mk (New.Array._induct α.1) (New.Array._encoding α.1 α.2)
+  fun _ α_extra => .mk (New.Array._induct α_extra.1) (New.Array._encoding α_extra.1 α_extra.2)
     (IsPropEncodingTrivial.univElim.{u + 1} _)
 
 def New.Array.mk : new_type% @Array.mk.{u} :=
@@ -227,9 +228,9 @@ def New.Array.rec.{u, v} : new_type% @Array.rec.{u, v} :=
 
 convert_to_new String
 
-instance {α_base : Type u} {α : new_type% α_base} [SubsingletonExtra α] :
-    SubsingletonExtra (New.List α) where
-  subsingleton t_base := by
+instance {α : Type u} {α_extra : new_type% α} [SubsingletonExtra α_extra] :
+    SubsingletonExtra (new% List α) where
+  subsingleton t := by
     constructor
     intro t₁ t₂
     induction t₁ with
@@ -240,120 +241,121 @@ instance {α_base : Type u} {α : new_type% α_base} [SubsingletonExtra α] :
       cases ih tail'
       rfl
 
-instance {α_base : Type u} {α : new_type% α_base} [InhabitedExtra α] :
-    InhabitedExtra (New.List α) where
-  default t_base := t_base.rec .nil fun head _ ih => .cons (InhabitedExtra.default head) ih
+instance {α : Type u} {α_extra : new_type% α} [InhabitedExtra α_extra] :
+    InhabitedExtra (new% List α) where
+  default t := t.rec .nil fun head _ ih => .cons (InhabitedExtra.default head) ih
 
-instance {α_base : Type u} {α : new_type% α_base} [SubsingletonExtra α] :
-    SubsingletonExtra (New.Array α) where
-  subsingleton t_base := by
+instance {α : Type u} {α_extra : new_type% α} [SubsingletonExtra α_extra] :
+    SubsingletonExtra (new% Array α) where
+  subsingleton t := by
     constructor
     intro t₁ t₂
     refine congrArg New.Array._induct.mk ?_
-    apply Subsingleton.allEq (α := new_type% t_base.1)
+    apply Subsingleton.allEq (α := new_type% t.1)
 
-instance {α_base : Type u} {α : new_type% α_base} [InhabitedExtra α] :
-    InhabitedExtra (New.Array α) where
-  default t_base := t_base.rec fun a => .mk (InhabitedExtra.default (α := New.List α) a)
+instance {α : Type u} {α_extra : new_type% α} [InhabitedExtra α_extra] :
+    InhabitedExtra (new% Array α) where
+  default t := t.rec fun a => .mk (InhabitedExtra.default (α_extra := new% List α) a)
 
-def inhabitedExtraOfDecidable {p_base : Prop} {p : new_type% p_base}
-    {h_base : Decidable p_base} (h : new_type% h_base) :
-    InhabitedExtra p where
-  default t_base := by cases h <;> trivial
+def inhabitedExtraOfDecidable {p : Prop} {p_extra : new_type% p}
+    {h : Decidable p} (h_extra : new_type% h) :
+    InhabitedExtra p_extra where
+  default t := by cases h_extra <;> trivial
 
-instance {n_base : ℕ} {n : new_type% n_base} {m_base : ℕ} {m : new_type% m_base} :
-    InhabitedExtra (@New.Nat.le n_base n m_base m) :=
-  inhabitedExtraOfDecidable (new% Nat.decLe n_base m_base)
+instance {n : ℕ} {n_extra : new_type% n} {m : ℕ} {m_extra : new_type% m} :
+    InhabitedExtra (new% Nat.le n m) :=
+  inhabitedExtraOfDecidable (new% Nat.decLe n m)
 
-instance {n_base : ℕ} {n : new_type% n_base} {m_base : ℕ} {m : new_type% m_base} :
-    InhabitedExtra (new% n_base ≤ m_base) :=
-  inferInstanceAs (InhabitedExtra (new% Nat.le n_base m_base))
+instance {n : ℕ} {n_extra : new_type% n} {m : ℕ} {m_extra : new_type% m} :
+    InhabitedExtra (new% n ≤ m) :=
+  inferInstanceAs (InhabitedExtra (new% Nat.le n m))
 
-instance {n_base : ℕ} {n : new_type% n_base} {m_base : ℕ} {m : new_type% m_base} :
-    InhabitedExtra (new% n_base < m_base) :=
-  inferInstanceAs (InhabitedExtra (new% Nat.le n_base.succ m_base))
+instance {n : ℕ} {n_extra : new_type% n} {m : ℕ} {m_extra : new_type% m} :
+    InhabitedExtra (new% n < m) :=
+  inferInstanceAs (InhabitedExtra (new% Nat.le n.succ m))
 
-instance {n_base : ℕ} {n : new_type% n_base} : InhabitedExtra (@New.Fin n_base n) where
-  default t_base :=
-    .mk _ _ () (InhabitedExtra.default (α := @New.Nat.le t_base.succ () n_base ()) t_base.2)
+instance {n : ℕ} {n_extra : new_type% n} : InhabitedExtra (new% Fin n) where
+  default t :=
+    .mk _ _ () (InhabitedExtra.default (α_extra := @New.Nat.le t.succ () n ()) t.2)
 
-instance {n_base : ℕ} {n : new_type% n_base} : SubsingletonExtra (@New.Fin n_base n) where
-  subsingleton t_base := by
+instance {n : ℕ} {n_extra : new_type% n} : SubsingletonExtra (new% Fin n) where
+  subsingleton t := by
     constructor
     rintro ⟨⟩ ⟨⟩; rfl
 
-instance {n_base : ℕ} {n : new_type% n_base} : InhabitedExtra (@New.BitVec n_base n) where
-  default t_base := .ofFin _ _ (InhabitedExtra.default (α := new% Fin (Nat.pow 2 n_base)) t_base.1)
+instance {n : ℕ} {n_extra : new_type% n} : InhabitedExtra (new% BitVec n) where
+  default t := .ofFin _ _ (InhabitedExtra.default (α_extra := new% Fin (Nat.pow 2 n)) t.1)
 
-instance {n_base : ℕ} {n : new_type% n_base} : SubsingletonExtra (@New.BitVec n_base n) where
-  subsingleton t_base := by
+instance {n : ℕ} {n_extra : new_type% n} : SubsingletonExtra (@New.BitVec n n_extra) where
+  subsingleton t := by
     constructor
     rintro ⟨⟨⟩⟩ ⟨⟨⟩⟩; rfl
 
 instance : InhabitedExtra New.UInt8 where
-  default t_base := .ofBitVec _ (InhabitedExtra.default (α := new% BitVec 8) t_base.1)
+  default t := .ofBitVec _ (InhabitedExtra.default (α_extra := new% BitVec 8) t.1)
 
 instance : SubsingletonExtra New.UInt8 where
-  subsingleton t_base := by
+  subsingleton t := by
     constructor
     rintro ⟨⟨⟨⟩⟩⟩ ⟨⟨⟨⟩⟩⟩; rfl
 
 instance : InhabitedExtra New.UInt32 where
-  default t_base := .ofBitVec _ (InhabitedExtra.default (α := new% BitVec 32) t_base.1)
+  default t := .ofBitVec _ (InhabitedExtra.default (α_extra := new% BitVec 32) t.1)
 
 instance : SubsingletonExtra New.UInt32 where
-  subsingleton t_base := by
+  subsingleton t := by
     constructor
     rintro ⟨⟨⟨⟩⟩⟩ ⟨⟨⟨⟩⟩⟩; rfl
 
 convert_to_new inferInstance instDecidableOr instDecidableAnd
 
-instance {n_base : UInt32} (n : new_type% n_base) :
-    InhabitedExtra (New.UInt32.isValidChar n) :=
-  inhabitedExtraOfDecidable (new% (inferInstance : Decidable (UInt32.isValidChar n_base)))
+instance {n : UInt32} (n_extra : new_type% n) :
+    InhabitedExtra (new% UInt32.isValidChar n) :=
+  inhabitedExtraOfDecidable (new% (inferInstance : Decidable (UInt32.isValidChar n)))
 
 instance : InhabitedExtra New.Char where
-  default t_base := .mk _ (InhabitedExtra.default (α := New.UInt32) t_base.1)
-    (InhabitedExtra.default (α := @New.UInt32.isValidChar t_base.1 _) _)
+  default t := .mk _ (InhabitedExtra.default (α_extra := New.UInt32) t.1)
+    (InhabitedExtra.default (α_extra := @New.UInt32.isValidChar t.1 _) _)
 
 instance : SubsingletonExtra New.Char where
-  subsingleton t_base := by
+  subsingleton t := by
     constructor
     rintro ⟨⟨⟨⟨⟩⟩⟩⟩ ⟨⟨⟨⟩⟩⟩; rfl
 
 instance : SubsingletonExtra New.ByteArray where
-  subsingleton t_base := by
+  subsingleton t := by
     constructor
     rintro ⟨a⟩ ⟨b⟩
     cases Subsingleton.allEq a b; rfl
 
 instance : InhabitedExtra New.ByteArray where
-  default t_base := t_base.rec fun a => .mk _
-    (show new_type% a from InhabitedExtra.default (α := New.Array New.UInt8) a)
+  default t := t.rec fun a => .mk _
+    (show new_type% a from InhabitedExtra.default (α_extra := New.Array New.UInt8) a)
 
-instance {b_base : ByteArray} (b : new_type% b_base) :
-    InhabitedExtra (New.ByteArray.IsValidUTF8 b) where
-  default t_base := by
-    rcases t_base with ⟨l, hl⟩
+instance {b : ByteArray} (b_extra : new_type% b) :
+    InhabitedExtra (New.ByteArray.IsValidUTF8 b_extra) where
+  default t := by
+    rcases t with ⟨l, hl⟩
     refine @New.ByteArray.IsValidUTF8._induct.intro _ _ l ?_ hl ?_
     · with_reducible exact InhabitedExtra.default _
     · with_reducible exact InhabitedExtra.default _
 
 instance : SubsingletonExtra New.String where
-  subsingleton t_base := by
+  subsingleton t := by
     constructor
     rintro ⟨a⟩ ⟨b⟩
     cases Subsingleton.allEq a b; rfl
 
 instance : InhabitedExtra New.String where
-  default t_base := .ofByteArray _ (InhabitedExtra.default (α := New.ByteArray) _)
-    (InhabitedExtra.default (α := @New.ByteArray.IsValidUTF8 t_base.1 _) _)
+  default t := .ofByteArray _ (InhabitedExtra.default (α_extra := New.ByteArray) _)
+    (InhabitedExtra.default (α_extra := @New.ByteArray.IsValidUTF8 t.1 _) _)
 
 noncomputable def uniqueStrVal (s : String) : new_type% s :=
-  InhabitedExtra.default (α := new% String) s
+  InhabitedExtra.default (α_extra := new% String) s
 
-instance {p_base : Prop} {p : new_type% p_base} {q_base : Prop} {q : new_type% q_base}
-    [InhabitedExtra p] [InhabitedExtra q] : InhabitedExtra (New.Iff p q) where
+instance {p : Prop} {p_extra : new_type% p} {q : Prop} {q_extra : new_type% q}
+    [InhabitedExtra p_extra] [InhabitedExtra q_extra] :
+    InhabitedExtra (New.Iff p_extra q_extra) where
   default h := by
     constructor
     · intro hp hp'
@@ -361,15 +363,17 @@ instance {p_base : Prop} {p : new_type% p_base} {q_base : Prop} {q : new_type% q
     · intro hq hq'
       exact InhabitedExtra.default (h.mpr hq)
 
-instance {p_base : Prop} {p : new_type% p_base} {q_base : Prop} {q : new_type% q_base}
-    [InhabitedExtra p] [InhabitedExtra q] : InhabitedExtra (New.And p q) where
+instance {p : Prop} {p_extra : new_type% p} {q : Prop} {q_extra : new_type% q}
+    [InhabitedExtra p_extra] [InhabitedExtra q_extra] :
+    InhabitedExtra (New.And p_extra q_extra) where
   default h := by
     constructor
     · exact InhabitedExtra.default h.1
     · exact InhabitedExtra.default h.2
 
-instance {p_base : Prop} {p : new_type% p_base} {q_base : Prop} {q : new_type% q_base}
-    [InhabitedExtra p] [InhabitedExtra q] : InhabitedExtra (New.Or p q) where
+instance {p : Prop} {p_extra : new_type% p} {q : Prop} {q_extra : new_type% q}
+    [InhabitedExtra p_extra] [InhabitedExtra q_extra] :
+    InhabitedExtra (New.Or p_extra q_extra) where
   default h := by
     rcases h with h | h
     · left; exact InhabitedExtra.default h
@@ -380,48 +384,50 @@ convert_to_new Lean.SourceInfo Lean.SyntaxNodeKind Lean.Syntax.Preresolved
 inductive _root_.New.Lean.Syntax._induct : Lean.Syntax → Type where
   | missing : _induct .missing
   | node
-    {info_base : Lean.SourceInfo} (info : new_type% info_base)
-    {kind_base : Lean.SyntaxNodeKind} (kind : new_type% kind_base)
-    {args_base : Array Lean.Syntax}
-    (args : @New.List._induct Lean.Syntax _induct args_base.1) :
-    _induct (.node info_base kind_base args_base)
-  | atom {info_base : Lean.SourceInfo} (info : new_type% info_base)
-    {val_base : String} (val : new_type% val_base) : _induct (.atom info_base val_base)
-  | ident {info_base : Lean.SourceInfo} (info : new_type% info_base)
-    {rawVal_base : Substring.Raw} (rawVal : new_type% rawVal_base)
-    {val_base : Lean.Name} (val : new_type% val_base)
-    {preresolved_base : List Lean.Syntax.Preresolved}
-    (preresolved : new_type% preresolved_base) :
-    _induct (.ident info_base rawVal_base val_base preresolved_base)
+    {info : Lean.SourceInfo} (info_extra : new_type% info)
+    {kind : Lean.SyntaxNodeKind} (kind_extra : new_type% kind)
+    {args : Array Lean.Syntax}
+    (args_extra : @New.List._induct Lean.Syntax _induct args.1) :
+    _induct (.node info kind args)
+  | atom {info : Lean.SourceInfo} (info_extra : new_type% info)
+    {val : String} (val_extra : new_type% val) : _induct (.atom info val)
+  | ident {info : Lean.SourceInfo} (info_extra : new_type% info)
+    {rawVal : Substring.Raw} (rawVal_extra : new_type% rawVal)
+    {val : Lean.Name} (val_extra : new_type% val)
+    {preresolved : List Lean.Syntax.Preresolved}
+    (preresolved_extra : new_type% preresolved) :
+    _induct (.ident info rawVal val preresolved)
 
 inductive _root_.New.Lean.Syntax._encoding :
-    ⦃t_base : Lean.Syntax⦄ → New.Lean.Syntax._induct t_base → ℕ → Prop where
+    ⦃t : Lean.Syntax⦄ → New.Lean.Syntax._induct t → ℕ → Prop where
   | missing : _encoding .missing 1
   | node
-    {info_base : Lean.SourceInfo} {info : new_type% info_base}
-    {info_n : ℕ} (info_enc : New.Lean.SourceInfo.2 info info_n)
-    {kind_base : Lean.SyntaxNodeKind} {kind : new_type% kind_base}
-    {kind_n : ℕ} (kind_enc : New.Lean.SyntaxNodeKind.2 kind kind_n)
-    {args_base : Array Lean.Syntax}
-    {args : @New.List._induct Lean.Syntax New.Lean.Syntax._induct args_base.1}
-    {args_n : ℕ} (args_enc : New.List._encoding New.Lean.Syntax._induct _encoding args args_n) :
-    _encoding (.node info kind args) (Nat.pair (Nat.pair info_n kind_n) args_n * 4 + 2)
-  | atom {info_base : Lean.SourceInfo} {info : new_type% info_base}
-    {info_n : ℕ} (info_enc : New.Lean.SourceInfo.2 info info_n)
-    {val_base : String} {val : new_type% val_base}
-    {val_n : ℕ} (val_enc : New.String.2 val val_n) :
-    _encoding (.atom info val) (Nat.pair info_n val_n * 4 + 3)
-  | ident  {info_base : Lean.SourceInfo} {info : new_type% info_base}
-    {info_n : ℕ} (info_enc : New.Lean.SourceInfo.2 info info_n)
-    {rawVal_base : Substring.Raw} {rawVal : new_type% rawVal_base}
-    {rawVal_n : ℕ} (rawVal_enc : New.Substring.Raw.2 rawVal rawVal_n)
-    {val_base : Lean.Name} (val : new_type% val_base)
-    {val_n : ℕ} (val_enc : New.Lean.Name.2 val val_n)
-    {preresolved_base : List Lean.Syntax.Preresolved}
-    (preresolved : new_type% preresolved_base)
+    {info : Lean.SourceInfo} {info_extra : new_type% info}
+    {info_n : ℕ} (info_enc : New.Lean.SourceInfo.2 info_extra info_n)
+    {kind : Lean.SyntaxNodeKind} {kind_extra : new_type% kind}
+    {kind_n : ℕ} (kind_enc : New.Lean.SyntaxNodeKind.2 kind_extra kind_n)
+    {args : Array Lean.Syntax}
+    {args_extra : @New.List._induct Lean.Syntax New.Lean.Syntax._induct args.1}
+    {args_n : ℕ} (args_enc : New.List._encoding
+      New.Lean.Syntax._induct _encoding args_extra args_n) :
+    _encoding (.node info_extra kind_extra args_extra)
+      (Nat.pair (Nat.pair info_n kind_n) args_n * 4 + 2)
+  | atom {info : Lean.SourceInfo} {info_extra : new_type% info}
+    {info_n : ℕ} (info_enc : New.Lean.SourceInfo.2 info_extra info_n)
+    {val : String} {val_extra : new_type% val}
+    {val_n : ℕ} (val_enc : New.String.2 val_extra val_n) :
+    _encoding (.atom info_extra val_extra) (Nat.pair info_n val_n * 4 + 3)
+  | ident  {info : Lean.SourceInfo} {info_extra : new_type% info}
+    {info_n : ℕ} (info_enc : New.Lean.SourceInfo.2 info_extra info_n)
+    {rawVal : Substring.Raw} {rawVal_extra : new_type% rawVal}
+    {rawVal_n : ℕ} (rawVal_enc : New.Substring.Raw.2 rawVal_extra rawVal_n)
+    {val : Lean.Name} (val_extra : new_type% val)
+    {val_n : ℕ} (val_enc : New.Lean.Name.2 val_extra val_n)
+    {preresolved : List Lean.Syntax.Preresolved}
+    (preresolved_extra : new_type% preresolved)
     {preresolved_n : ℕ}
-    (preresolved_enc : (New.List New.Lean.Syntax.Preresolved).2 preresolved preresolved_n) :
-    _encoding (.ident info rawVal val preresolved)
+    (preresolved_enc : (New.List New.Lean.Syntax.Preresolved).2 preresolved_extra preresolved_n) :
+    _encoding (.ident info_extra rawVal_extra val_extra preresolved_extra)
       (Nat.pair (Nat.pair (Nat.pair info_n rawVal_n) val_n) preresolved_n * 4 + 4)
 
 def New.Lean.Syntax : new_type% Lean.Syntax :=
@@ -434,28 +440,28 @@ def New.Lean.Syntax.node : new_type% Lean.Syntax.node :=
   fun _ info _ kind _ args => _induct.node info kind args.1
 
 noncomputable def New.Lean.Syntax.rec : new_type% @Lean.Syntax.rec.{u} :=
-  fun motive_1_base motive_1 motive_2_base _ motive_3_base motive_3
-      missing_base missing node_base node atom_base atom ident_base ident
-      mk_base mk nil_base nil cons_base cons t_base t =>
-    @Syntax._induct.rec (fun t_base t => (motive_1 t).1
-        (@_root_.Lean.Syntax.rec motive_1_base motive_2_base motive_3_base
-          missing_base node_base atom_base ident_base mk_base nil_base cons_base t_base))
-      (fun t_base t => (motive_3 t).1
-        (@Lean.Syntax.rec_2 motive_1_base motive_2_base motive_3_base
-          missing_base node_base atom_base ident_base mk_base nil_base cons_base t_base))
-      missing
-      (fun _ _ _ _ _ ih => node _ _ _ (mk _ ih))
-      @atom @ident @nil
-      (fun _ _ _ head_ih tail_ih => cons _ _ head_ih tail_ih)
-      t_base t
+  fun motive_1 motive_1_extra motive_2 _ motive_3 motive_3_extra
+      missing missing_extra node node_extra atom atom_extra ident ident_extra
+      mk mk_extra nil nil_extra cons cons_extra t t_extra =>
+    @Syntax._induct.rec (fun t t_extra => (motive_1_extra t_extra).1
+        (@_root_.Lean.Syntax.rec motive_1 motive_2 motive_3
+          missing node atom ident mk nil cons t))
+      (fun t t_extra => (motive_3_extra t_extra).1
+        (@Lean.Syntax.rec_2 motive_1 motive_2 motive_3
+          missing node atom ident mk nil cons t))
+      missing_extra
+      (fun _ _ _ _ _ ih => node_extra _ _ _ (mk_extra _ ih))
+      @atom_extra @ident_extra @nil_extra
+      (fun _ _ _ head_ih tail_ih => cons_extra _ _ head_ih tail_ih)
+      t t_extra
 
 convert_to_new Prod
 
-instance {α_base : Type u} (α : new_type% α_base)
-    {β_base : Type v} (β : new_type% β_base)
-    [SubsingletonExtra α] [SubsingletonExtra β] :
-    SubsingletonExtra (New.Prod α β) where
-  subsingleton t_base := by
+instance {α : Type u} (α_extra : new_type% α)
+    {β : Type v} (β_extra : new_type% β)
+    [SubsingletonExtra α_extra] [SubsingletonExtra β_extra] :
+    SubsingletonExtra (New.Prod α_extra β_extra) where
+  subsingleton t := by
     constructor
     rintro ⟨a, b⟩ ⟨a', b'⟩
     cases Subsingleton.allEq a a'
@@ -487,9 +493,9 @@ theorem almostEm (p : Prop) : p ∨ (p ↔ Middle) ∨ ¬p := by
   · exact .inr (.inr h)
 
 theorem New.almostEm : new_type% almostEm := by
-  intro p_base p
-  by_cases h : p_base
-  · by_cases h' : p.1 h
+  intro p p_extra
+  by_cases h : p
+  · by_cases h' : p_extra.1 h
     · exact .inl h'
     · have iff := iff_of_true h Middle.intro
       refine @New.Or._induct.inr _ _ _ _ (.inl iff) ?_
