DependentComputability/SortExtra.lean
@@ -19,39 +19,39 @@ theorem isProp_of_isProp_imax.{u, v} (h : IsProp.{imax u v}) : IsProp.{v} := by
 
 @[mk_iff]
 inductive TrivialEncoding {α : Sort u} (Extra : α → Sort u) :
-    ⦃a_base : α⦄ → (a : Extra a_base) → (n : ℕ) → Prop where
-  | zero {a_base} {a : Extra a_base} : TrivialEncoding Extra a 0
+    ⦃a : α⦄ → (a : Extra a) → (n : ℕ) → Prop where
+  | zero {a} {a_extra : Extra a} : TrivialEncoding Extra a_extra 0
 
 attribute [simp] trivialEncoding_iff
 
 def IsPropEncodingTrivial {α : Sort u} {Extra : α → Sort u}
-    (Encoding : ∀ ⦃a_base : α⦄, Extra a_base → ℕ → Prop) : Prop :=
-  IsProp.{u} → ∀ {a_base} a n, @Encoding a_base a n ↔ TrivialEncoding Extra a n
+    (Encoding : ∀ ⦃a : α⦄, Extra a → ℕ → Prop) : Prop :=
+  IsProp.{u} → ∀ {a} a_extra n, @Encoding a a_extra n ↔ TrivialEncoding Extra a_extra n
 
 theorem IsPropEncodingTrivial.trivialEncoding {α : Sort u} (Extra : α → Sort u) :
     IsPropEncodingTrivial (TrivialEncoding Extra) := by
   intro; simp
 
 theorem IsPropEncodingTrivial.eq_of_isProp {α : Sort u} {Extra : α → Sort u}
-    {Encoding : ∀ ⦃a_base : α⦄, Extra a_base → ℕ → Prop}
+    {Encoding : ∀ ⦃a : α⦄, Extra a → ℕ → Prop}
     (h : IsPropEncodingTrivial Encoding) (hprop : IsProp.{u}) :
     Encoding = TrivialEncoding Extra := by
-  ext a_base a n
+  ext a a n
   apply h hprop
 
 theorem IsPropEncodingTrivial.eq {α : Prop} {Extra : α → Prop}
-    {Encoding : ∀ ⦃a_base : α⦄, Extra a_base → ℕ → Prop}
+    {Encoding : ∀ ⦃a : α⦄, Extra a → ℕ → Prop}
     (h : IsPropEncodingTrivial Encoding) :
     Encoding = TrivialEncoding Extra := h.eq_of_isProp isProp_prop
 
 theorem IsPropEncodingTrivial.univElim {α : Sort (max 1 u)} {Extra : α → Sort (max 1 u)}
-    (Encoding : ∀ ⦃a_base : α⦄, Extra a_base → ℕ → Prop) :
+    (Encoding : ∀ ⦃a : α⦄, Extra a → ℕ → Prop) :
     @IsPropEncodingTrivial α Extra Encoding := by
   intro h
   exact absurd h not_isProp.{u}
 
 inductive SortExtra (α : Sort u) where
-  | mk (Extra : α → Sort u) (Encoding : ∀ ⦃a_base : α⦄ (_ : Extra a_base), ℕ → Prop)
+  | mk (Extra : α → Sort u) (Encoding : ∀ ⦃a : α⦄, Extra a → ℕ → Prop)
     (propElim : IsPropEncodingTrivial Encoding)
 
 theorem IsProp.encoding_eq {x : SortExtra.{u} α} (hprop : IsProp.{u}) :
@@ -63,21 +63,22 @@ def New.«Sort».{u} : SortExtra (Sort u) :=
     (IsPropEncodingTrivial.trivialEncoding SortExtra)
 
 inductive ForallEncoding
-    {α_base : Sort u} (α : New.Sort.{u}.1 α_base) {β_base : α_base → Sort v}
-    (β : ∀ ⦃a_base : α_base⦄, ∀ _ : α.1 a_base, New.Sort.{v}.1 (β_base a_base))
-    ⦃f_base : (a : α_base) → β_base a⦄
-    (f : ∀ ⦃a_base : α_base⦄ (a : α.1 a_base), (β a).1 (f_base a_base)) :
+    {α : Sort u} (α_extra : New.Sort.{u}.1 α) {β : α → Sort v}
+    (β_extra : ∀ ⦃a : α⦄, ∀ _ : α_extra.1 a, New.Sort.{v}.1 (β a))
+    ⦃f : (a : α) → β a⦄
+    (f_extra : ∀ ⦃a : α⦄ (a_extra : α_extra.1 a), (β_extra a_extra).1 (f a)) :
     ℕ → Prop where
-  | zero (hprop : IsProp.{imax u v}) : ForallEncoding α β f 0
+  | zero (hprop : IsProp.{imax u v}) : ForallEncoding α_extra β_extra f_extra 0
   | encode (hprop : ¬IsProp.{imax u v}) (code : Nat.Partrec.Code)
-    (hcode : ∀ ⦃a_base a n⦄, @α.2 a_base a n → ∃ m ∈ code.eval n, (β a).2 (f a) m) :
-    ForallEncoding α β f (Encodable.encode code)
+    (hcode : ∀ ⦃a a_extra n⦄, @α_extra.2 a a_extra n →
+      ∃ m ∈ code.eval n, (β_extra a_extra).2 (f_extra a_extra) m) :
+    ForallEncoding α_extra β_extra f_extra (Encodable.encode code)
 
 theorem IsPropEncodingTrivial.forallEncoding
-    {α_base : Sort u} (α : New.Sort.{u}.1 α_base) {β_base : α_base → Sort v}
-    (β : ∀ ⦃a_base : α_base⦄, ∀ _ : α.1 a_base, New.Sort.{v}.1 (β_base a_base)) :
-    IsPropEncodingTrivial (ForallEncoding α β) := by
-  intro hprop a_base a n
+    {α : Sort u} (α_extra : New.Sort.{u}.1 α) {β : α → Sort v}
+    (β_extra : ∀ ⦃a : α⦄, ∀ _ : α_extra.1 a, New.Sort.{v}.1 (β a)) :
+    IsPropEncodingTrivial (ForallEncoding α_extra β_extra) := by
+  intro hprop a a n
   constructor
   · rintro (⟨⟩ | ⟨h⟩)
     · constructor
@@ -87,11 +88,11 @@ theorem IsPropEncodingTrivial.forallEncoding
     assumption
 
 def New.«Forall».{u, v}
-    {α_base : Sort u} (α : New.Sort.{u}.1 α_base) {β_base : α_base → Sort v}
-    (β : ∀ ⦃a_base : α_base⦄, ∀ _ : α.1 a_base, New.Sort.{v}.1 (β_base a_base)) :
-    New.Sort.{imax u v}.1 ((a : α_base) → β_base a) :=
-  .mk (Extra := fun f => ∀ ⦃a_base : α_base⦄, ∀ a : α.1 a_base, (β a).1 (f a_base))
-    (Encoding := ForallEncoding α β) (propElim := .forallEncoding α β)
+    {α : Sort u} (α_extra : New.Sort.{u}.1 α) {β : α → Sort v}
+    (β_extra : ∀ ⦃a : α⦄, ∀ _ : α_extra.1 a, New.Sort.{v}.1 (β a)) :
+    New.Sort.{imax u v}.1 ((a : α) → β a) :=
+  .mk (Extra := fun f => ∀ ⦃a : α⦄, ∀ a_extra : α_extra.1 a, (β_extra a_extra).1 (f a))
+    (Encoding := ForallEncoding α_extra β_extra) (propElim := .forallEncoding α_extra β_extra)
 
 def mkNewName (nm : Lean.Name) : Lean.Name :=
   match nm with
@@ -109,9 +110,9 @@ abbrev mkExtraApp (ty e : Expr) : Expr :=
 
 open Lean Qq in
 @[inline]
-def mkExtraAppQ {α_base : Q(Sort u)} (α : Q(New.Sort.{u}.1 $α_base))
-    (x_base : Q($α_base)) : Q(Sort u) :=
-  q($α.1 $x_base)
+def mkExtraAppQ {α : Q(Sort u)} (α_extra : Q(New.Sort.{u}.1 $α))
+    (x : Q($α)) : Q(Sort u) :=
+  q($α_extra.1 $x)
 
 open Lean in
 initialize declConverterRef : IO.Ref (Name → CoreM Unit) ← IO.mkRef fun _ => pure ()
@@ -169,72 +170,72 @@ def isStructureLikeWithLargeElim (nm : Name) : CoreM Bool := do
 
 open Lean Meta in
 partial def conversionStepNew (e : Expr) : MetaM Expr := do
-  let rec visit (e : Expr) (baseMap : FVarIdMap Expr) : MonadCacheT ExprStructEq Expr MetaM Expr :=
+  let rec visit (e : Expr) (extraMap : FVarIdMap Expr) : MonadCacheT ExprStructEq Expr MetaM Expr :=
     withTraceNode `debug (fun err => return m!"{exceptEmoji err} Transforming {e}") do
     checkCache { val := e : ExprStructEq } fun _ => Meta.withIncRecDepth do
       match e with
       | .lit (.natVal _) => return .app (.const `uniqueNatVal []) e
       | .lit (.strVal _) => return .app (.const `uniqueStrVal []) e
       | .fvar f =>
-        let some val := baseMap.get? f |
+        let some val := extraMap.get? f |
           throwError "invalid variable: {e} in\n{(← mkFreshExprMVar none).mvarId!}"
         return val
       | .mvar _ => throwError "unexpected metavariable"
       | .bvar _ => throwError "unexpected bound variable"
-      | .mdata m e => return .mdata m (← visit e baseMap)
+      | .mdata m e => return .mdata m (← visit e extraMap)
       | .proj t i e =>
         if ← isStructureLikeWithLargeElim t then
-          return .proj (mkNewInductName t) i (← visit e baseMap)
+          return .proj (mkNewInductName t) i (← visit e extraMap)
         else
           conversionStepNew (← projToRec t i e)
-      | .app f a => return mkApp2 (← visit f baseMap) a (← visit a baseMap)
+      | .app f a => return mkApp2 (← visit f extraMap) a (← visit a extraMap)
       | .letE nm t v b nd =>
-        let baseName := nm.appendAfter "_base"
-        withLetDecl baseName t v (nondep := false) fun baseVar => do
-          let newT ← visit t baseMap
+        withLetDecl nm t v (nondep := false) fun baseVar => do
+          let newT ← visit t extraMap
           let newT' := mkExtraApp newT (.bvar 0)
-          let newV ← visit v baseMap
-          withLetDecl nm newT' newV (nondep := nd) fun var => do
-            let newB ← visit (b.instantiate1 baseVar) (baseMap.insert baseVar.fvarId! var)
+          let newV ← visit v extraMap
+          let extraName := nm.appendAfter "_extra"
+          withLetDecl extraName newT' newV (nondep := nd) fun var => do
+            let newB ← visit (b.instantiate1 baseVar) (extraMap.insert baseVar.fvarId! var)
             let newB := newB.abstract #[baseVar, var]
-            return .letE baseName t v (.letE nm newT' newV newB nd) false
+            return .letE nm t v (.letE extraName newT' newV newB nd) false
       | .sort u => return .const ``New.Sort [u]
       | .const nm us => return .const (mkNewName nm) us
       | .forallE nm t b bi =>
         let u ← getLevel t
         let v ← withLocalDecl nm bi t fun a => getLevel (b.instantiate1 a)
-        let baseName := nm.appendAfter "_base"
-        withLocalDecl baseName bi t fun baseVar => do
-          let newT ← visit t baseMap
+        withLocalDecl nm bi t fun var => do
+          let newT ← visit t extraMap
           let newT' := mkExtraApp newT (.bvar 0)
-          withLocalDecl nm bi newT fun var => do
-            let newB ← visit (b.instantiate1 baseVar) (baseMap.insert baseVar.fvarId! var)
-            let newB := newB.abstract #[baseVar, var]
+          let extraName := nm.appendAfter "_extra"
+          withLocalDecl extraName bi newT fun extraVar => do
+            let newB ← visit (b.instantiate1 var) (extraMap.insert var.fvarId! extraVar)
+            let newB := newB.abstract #[var, extraVar]
             return mkApp4 (.const ``New.Forall [u, v]) t newT
-              (.lam nm t b bi) (.lam baseName t (.lam nm newT' newB bi)
+              (.lam nm t b bi) (.lam nm t (.lam extraName newT' newB bi)
                 (if bi.isImplicit then .implicit else .strictImplicit))
       | .lam nm t b bi =>
-        let baseName := nm.appendAfter "_base"
-        withLocalDecl baseName bi t fun baseVar => do
-          let newT ← visit t baseMap
+        withLocalDecl nm bi t fun var => do
+          let newT ← visit t extraMap
           let newT' := mkExtraApp newT (.bvar 0)
-          withLocalDecl nm bi newT fun var => do
-            let newB ← visit (b.instantiate1 baseVar) (baseMap.insert baseVar.fvarId! var)
-            let newB := newB.abstract #[baseVar, var]
-            return .lam baseName t (.lam nm newT' newB bi)
+          let extraName := nm.appendAfter "_extra"
+          withLocalDecl extraName bi newT fun extraVar => do
+            let newB ← visit (b.instantiate1 var) (extraMap.insert var.fvarId! extraVar)
+            let newB := newB.abstract #[var, extraVar]
+            return .lam nm t (.lam extraName newT' newB bi)
               (if bi.isImplicit then .implicit else .strictImplicit)
   (visit e {}).run
 
 open Lean Meta in
 def populateBaseMap : MetaM (FVarIdMap Expr) := do
   let lctx ← getLCtx
-  let mut baseMap : FVarIdMap Expr := {}
+  let mut extraMap : FVarIdMap Expr := {}
   for decl in lctx do
     let type := decl.type
     let type ← instantiateMVars type
     let mkExtraApp _ty (.fvar baseVar) := type | continue
-    baseMap := baseMap.insert baseVar decl.toExpr
-  return baseMap
+    extraMap := extraMap.insert baseVar decl.toExpr
+  return extraMap
 
 open Lean Elab Term in
 elab tk:"new% " t:term : term => do
@@ -247,9 +248,9 @@ elab tk:"new% " t:term : term => do
   let expr ← elabTerm t eTy
   synthesizeSyntheticMVarsNoPostponing
   let expr ← instantiateMVars expr
-  let baseMap ← populateBaseMap
-  if expr.hasAnyFVar (not ∘ baseMap.contains) then
-    let some a := expr.find? (fun | .fvar f => !baseMap.contains f | _ => false) |
+  let extraMap ← populateBaseMap
+  if expr.hasAnyFVar (not ∘ extraMap.contains) then
+    let some a := expr.find? (fun | .fvar f => !extraMap.contains f | _ => false) |
       throwErrorAt tk "expression has free variables"
     throwErrorAt tk "Invalid unresolved free variable {a} in{indentExpr expr}"
   if expr.hasMVar then
@@ -258,12 +259,12 @@ elab tk:"new% " t:term : term => do
     unless (← getEnv).contains (mkNewName const) do
       let converter ← declConverterRef.get
       converter const
-  let res ← (conversionStepNew.visit expr baseMap).run
+  let res ← (conversionStepNew.visit expr extraMap).run
   if let some expTy := expectedType? then
     let expTy ← instantiateMVars expTy
     let mkExtraApp ty val := expTy | return res
     let type ← Meta.inferType expr
-    let typeRes ← (conversionStepNew.visit type baseMap).run
+    let typeRes ← (conversionStepNew.visit type extraMap).run
     discard <| Meta.isDefEq ty typeRes
     discard <| Meta.isDefEq val expr
   return res
@@ -273,9 +274,9 @@ elab tk:"new_type% " t:term : term => do
   let expr ← elabTerm t none
   let type ← Meta.inferType expr
   let type ← instantiateMVars type
-  let baseMap ← populateBaseMap
-  if type.hasAnyFVar (not ∘ baseMap.contains) then
-    let some a := type.find? (fun | .fvar f => !baseMap.contains f | _ => false) |
+  let extraMap ← populateBaseMap
+  if type.hasAnyFVar (not ∘ extraMap.contains) then
+    let some a := type.find? (fun | .fvar f => !extraMap.contains f | _ => false) |
       throwErrorAt tk "expression has free variables"
     throwErrorAt tk "Invalid unresolved free variable {a} in{indentExpr type}"
   if type.hasMVar then
@@ -284,16 +285,16 @@ elab tk:"new_type% " t:term : term => do
     unless (← getEnv).contains (mkNewName const) do
       let converter ← declConverterRef.get
       converter const
-  let newExpr ← (conversionStepNew.visit type baseMap).run
+  let newExpr ← (conversionStepNew.visit type extraMap).run
   return mkExtraApp newExpr expr
 
-class InhabitedExtra {α_base : Sort u} (α : new_type% α_base) where
-  default : ∀ a, α.1 a
+class InhabitedExtra {α : Sort u} (α_extra : new_type% α) where
+  default : ∀ a, α_extra.1 a
 
-class SubsingletonExtra {α_base : Sort u} (α : new_type% α_base) where
-  subsingleton : ∀ a, Subsingleton (α.1 a)
+class SubsingletonExtra {α : Sort u} (α_extra : new_type% α) where
+  subsingleton : ∀ a, Subsingleton (α_extra.1 a)
 
-instance {α_base α} [@InhabitedExtra α_base α] (a : α_base) : Nonempty (new_type% a) :=
+instance {α α_extra} [@InhabitedExtra α α_extra] (a : α) : Nonempty (new_type% a) :=
   ⟨InhabitedExtra.default a⟩
 
 attribute [instance] SubsingletonExtra.subsingleton
@@ -301,63 +302,65 @@ attribute [instance] SubsingletonExtra.subsingleton
 instance : InhabitedExtra New.Sort.{u} where
   default _ := ⟨fun _ => PUnit.{u}, TrivialEncoding _, .trivialEncoding _⟩
 
-instance {α_base : Sort u} (α : New.Sort.1 α_base) {β_base : α_base → Sort v}
-    (β : ⦃a_base : α_base⦄ → α.1 a_base → New.Sort.1 (β_base a_base))
-    [∀ a_base a, InhabitedExtra (@β a_base a)] :
-    InhabitedExtra (New.Forall α β) where
-  default f a_base _ := InhabitedExtra.default (f a_base)
+instance {α : Sort u} (α_extra : new_type% α) {β : α → Sort v}
+    (β_extra : ⦃a : α⦄ → α_extra.1 a → New.Sort.1 (β a))
+    [∀ a a_extra, InhabitedExtra (@β_extra a a_extra)] :
+    InhabitedExtra (New.Forall α_extra β_extra) where
+  default f a _ := InhabitedExtra.default (f a)
 
-instance {α_base : Sort u} (α : New.Sort.1 α_base) {β_base : α_base → Sort v}
-    (β : ⦃a_base : α_base⦄ → α.1 a_base → New.Sort.1 (β_base a_base))
-    [∀ a_base a, SubsingletonExtra (@β a_base a)] :
-    SubsingletonExtra (New.Forall α β) where
+instance {α : Sort u} (α_extra : new_type% α) {β : α → Sort v}
+    (β_extra : ⦃a : α⦄ → α_extra.1 a → New.Sort.1 (β a))
+    [∀ a a_extra, SubsingletonExtra (@β_extra a a_extra)] :
+    SubsingletonExtra (New.Forall α_extra β_extra) where
   subsingleton f := by
     constructor
-    intro a_base a
-    funext x_base x
+    intro a a_extra
+    funext x x_extra
     apply Subsingleton.allEq
 
-instance (priority := low) {p_base : Prop} {p : new_type% p_base} : SubsingletonExtra p where
+instance (priority := low) {p : Prop} {p_extra : new_type% p} : SubsingletonExtra p_extra where
   subsingleton := inferInstance
 
-def IsRepresentable {α_base : Sort u} {α : new_type% α_base}
-    {x_base : α_base} (x : new_type% x_base) : Prop :=
-  ∃ n, α.2 x n
+def IsRepresentable {α : Sort u} {α_extra : new_type% α}
+    {x : α} (x_extra : new_type% x) : Prop :=
+  ∃ n, α_extra.2 x_extra n
 
-inductive DComputable {α_base : Sort u} {α : new_type% α_base}
-    {β_base : α_base → Sort v} {β : new_type% β_base}
-    {f_base : (a : α_base) → β_base a} (f : new_type% f_base) : Prop where
+inductive DComputable {α : Sort u} {α_extra : new_type% α}
+    {β : α → Sort v} {β_extra : new_type% β}
+    {f : (a : α) → β a} (f_extra : new_type% f) : Prop where
   | intro (g : ℕ →. ℕ) (hg : Nat.Partrec g)
-    (hg' : ∀ ⦃a_base a n⦄, @α.2 a_base a n → ∃ m ∈ g n, (β a).2 (f a) m)
+    (hg' : ∀ ⦃a a_extra n⦄, @α_extra.2 a a_extra n →
+      ∃ m ∈ g n, (β_extra a_extra).2 (f_extra a_extra) m)
 
-inductive DPrimrec {α_base : Sort u} {α : new_type% α_base}
-    {β_base : α_base → Sort v} {β : new_type% β_base}
-    {f_base : (a : α_base) → β_base a} (f : new_type% f_base) : Prop where
+inductive DPrimrec {α : Sort u} {α_extra : new_type% α}
+    {β : α → Sort v} {β_extra : new_type% β}
+    {f : (a : α) → β a} (f_extra : new_type% f) : Prop where
   | intro (g : ℕ → ℕ) (hg : Nat.Primrec g)
-    (hg' : ∀ ⦃a_base a n⦄, @α.2 a_base a n → (β a).2 (f a) (g n))
+    (hg' : ∀ ⦃a a_extra n⦄, @α_extra.2 a a_extra n → (β_extra a_extra).2 (f_extra a_extra) (g n))
 
-class FullyRepresentable {α_base : Sort u} (α : new_type% α_base)
-    extends InhabitedExtra α, SubsingletonExtra α where
-  isRepresentable : ∀ {x_base : α_base} (x : α.1 x_base), IsRepresentable x
+class FullyRepresentable {α : Sort u} (α_extra : new_type% α)
+    extends InhabitedExtra α_extra, SubsingletonExtra α_extra where
+  isRepresentable : ∀ {x : α} (x : α_extra.1 x), IsRepresentable x
 
-class CompatibleEncodingRelation {α_base : Type u} (α : new_type% α_base)
-    [Encodable α_base] extends FullyRepresentable α where
+class CompatibleEncodingRelation {α : Type u} (α_extra : new_type% α)
+    [Encodable α] extends FullyRepresentable α_extra where
   encode : ℕ → ℕ := id
   decode : ℕ → ℕ := id
   decode_encode (n : ℕ) : decode (encode n) = n := by intro; rfl
   encode_primrec : Nat.Primrec encode := by exact .id
   decode_primrec : Nat.Primrec decode := by exact .id
-  encode_eq {x_base : α_base} {x : α.1 x_base} {n : ℕ}
-      (hx : α.2 x n) : encode n = Encodable.encode x_base
+  encode_eq {x : α} {x_extra : α_extra.1 x} {n : ℕ}
+      (hx : α_extra.2 x_extra n) : encode n = Encodable.encode x
 
 attribute [simp] CompatibleEncodingRelation.decode_encode
 
-theorem encoding_pi_def {α_base : Sort u} {α : new_type% α_base}
-    {β_base : α_base → Sort v} {β : new_type% β_base}
+theorem encoding_pi_def {α : Sort u} {α_extra : new_type% α}
+    {β : α → Sort v} {β_extra : new_type% β}
     (h : ¬ IsProp.{imax u v})
-    {f_base : (a : α_base) → β_base a} (f : new_type% f_base) (n : ℕ) :
-    (new% ∀ a, β_base a).2 f n ↔ ∀ ⦃a_base a n₁⦄, @α.2 a_base a n₁ →
-      ∃ n₂ ∈ (Denumerable.ofNat Nat.Partrec.Code n).eval n₁, (β a).2 (f a) n₂ := by
+    {f : (a : α) → β a} (f_extra : new_type% f) (n : ℕ) :
+    (new% ∀ a, β a).2 f_extra n ↔ ∀ ⦃a a_extra n₁⦄, @α_extra.2 a a_extra n₁ →
+      ∃ n₂ ∈ (Denumerable.ofNat Nat.Partrec.Code n).eval n₁,
+        (β_extra a_extra).2 (f_extra a_extra) n₂ := by
   constructor
   · rintro (⟨⟩ | ⟨_, code, hcode⟩)
     · contradiction
@@ -366,10 +369,10 @@ theorem encoding_pi_def {α_base : Sort u} {α : new_type% α_base}
     rw [← Denumerable.encode_ofNat (α := Nat.Partrec.Code) n]
     exact .encode ‹_› _ h
 
-theorem isRepresentable_function_iff {α_base : Sort u} {α : new_type% α_base}
-    {β_base : α_base → Sort v} {β : new_type% β_base}
-    {f_base : (a : α_base) → β_base a} (f : new_type% f_base) :
-    IsRepresentable (new% f_base) ↔ DComputable f := by
+theorem isRepresentable_function_iff {α : Sort u} {α_extra : new_type% α}
+    {β : α → Sort v} {β_extra : new_type% β}
+    {f : (a : α) → β a} (f_extra : new_type% f) :
+    IsRepresentable (new% f) ↔ DComputable f_extra := by
   by_cases hprop : IsProp.{imax u v}
   · simp only [IsRepresentable, hprop.encoding_eq, trivialEncoding_iff,
       exists_eq, true_iff]
@@ -385,50 +388,50 @@ theorem isRepresentable_function_iff {α_base : Sort u} {α : new_type% α_base}
     use Encodable.encode c
     simpa using hg'
 
-class Irrelevant {α_base : Sort u} (α : new_type% α_base) where
-  encoding ⦃a_base : α_base⦄ (a : α.1 a_base) : α.2 a 0
+class Irrelevant {α : Sort u} (α_extra : new_type% α) where
+  encoding ⦃a : α⦄ (a : α_extra.1 a) : α_extra.2 a 0
 
 instance instIrrelevantSort : Irrelevant New.Sort.{u} where
   encoding _ _ := .zero
 
-instance (priority := low) {p_base : Prop} (p : New.Sort.{0}.1 p_base) : Irrelevant p where
+instance (priority := low) {p : Prop} (p : New.Sort.{0}.1 p) : Irrelevant p where
   encoding _ _ := (p.3 isProp_prop _ _).mpr .zero
 
 open Nat.Partrec Code in
-instance instIrrelevantForall {α_base : Sort u} (α : New.Sort.1 α_base) {β_base : α_base → Sort v}
-    (β : ⦃a_base : α_base⦄ → α.1 a_base → New.Sort.1 (β_base a_base))
-    [∀ ⦃a_base : α_base⦄ (a : α.1 a_base), Irrelevant (β a)] :
-    Irrelevant (New.Forall α β) where
-  encoding f_base f := by
+instance instIrrelevantForall {α : Sort u} (α_extra : new_type% α) {β : α → Sort v}
+    (β_extra : ⦃a : α⦄ → α_extra.1 a → New.Sort.1 (β a))
+    [∀ ⦃a : α⦄ (a : α_extra.1 a), Irrelevant (β_extra a)] :
+    Irrelevant (New.Forall α_extra β_extra) where
+  encoding f f := by
     by_cases hprop : IsProp.{imax u v}
     · exact .zero hprop
     rw [encoding_pi_def hprop]
     intros
     simp [ofNatCode_eq, ofNatCode, eval, pure, PFun.pure, Irrelevant.encoding]
 
-structure Encoding {α_base : Sort u} (α : new_type% α_base) where
+structure Encoding {α : Sort u} (α_extra : new_type% α) where
   repr : ℕ
 
 open CompatibleEncodingRelation in
-instance {α_base : Type u} {α : new_type% α_base} [Encodable α_base]
-    [CompatibleEncodingRelation α] : Primcodable (Encoding α) where
-  encode x := encode α x.repr
-  decode n := some ⟨decode α n⟩
+instance {α : Type u} {α_extra : new_type% α} [Encodable α]
+    [CompatibleEncodingRelation α_extra] : Primcodable (Encoding α_extra) where
+  encode x := encode α_extra x.repr
+  decode n := some ⟨decode α_extra n⟩
   encodek := by simp
   prim := .comp .succ (.comp encode_primrec decode_primrec)
 
-theorem Encoding.encode_eq {α_base : Type u} {α : new_type% α_base}
-    [Encodable α_base] [CompatibleEncodingRelation α]
-    {x_base : α_base} {x : new_type% x_base} {n : ℕ} (h : α.2 x n) :
-    Encodable.encode (⟨n⟩ : Encoding α) = Encodable.encode x_base :=
+theorem Encoding.encode_eq {α : Type u} {α_extra : new_type% α}
+    [Encodable α] [CompatibleEncodingRelation α_extra]
+    {x : α} {x_extra : new_type% x} {n : ℕ} (h : α_extra.2 x_extra n) :
+    Encodable.encode (⟨n⟩ : Encoding α_extra) = Encodable.encode x :=
   CompatibleEncodingRelation.encode_eq h
 
 theorem CompatibleEncodingRelation.encoding_unique
-    {α_base : Type u} {α : new_type% α_base}
-    [Encodable α_base] [CompatibleEncodingRelation α]
-    {x_base : α_base} {x : new_type% x_base}
-    {y_base : α_base} {y : new_type% y_base}
-    {n : ℕ} (hx : α.2 x n) (hy : α.2 y n) : x_base = y_base := by
+    {α : Type u} {α_extra : new_type% α}
+    [Encodable α] [CompatibleEncodingRelation α_extra]
+    {x : α} {x_extra : new_type% x}
+    {y : α} {y_extra : new_type% y}
+    {n : ℕ} (hx : α_extra.2 x_extra n) (hy : α_extra.2 y_extra n) : x = y := by
   apply Encodable.encode_injective
   rw [← Encoding.encode_eq hx, ← Encoding.encode_eq hy]
 
@@ -436,56 +439,56 @@ theorem Option.rec_eq_elim {α : Type u} {β : Type v} (x : Option α) (n : β) 
     Option.rec n s x = Option.elim x n s := by
   cases x <;> rfl
 
-theorem Encoding.primrec_mk {α_base : Type u} {α : new_type% α_base}
-    [Encodable α_base] [CompatibleEncodingRelation α] :
-    Primrec (Encoding.mk : ℕ → Encoding α) :=
+theorem Encoding.primrec_mk {α : Type u} {α_extra : new_type% α}
+    [Encodable α] [CompatibleEncodingRelation α_extra] :
+    Primrec (Encoding.mk : ℕ → Encoding α_extra) :=
   Nat.Primrec.comp .succ CompatibleEncodingRelation.encode_primrec
 
-theorem Encoding.primrec_repr {α_base : Type u} {α : new_type% α_base}
-    [Encodable α_base] [CompatibleEncodingRelation α] :
-    Primrec (Encoding.repr : Encoding α → ℕ) :=
+theorem Encoding.primrec_repr {α : Type u} {α_extra : new_type% α}
+    [Encodable α] [CompatibleEncodingRelation α_extra] :
+    Primrec (Encoding.repr : Encoding α_extra → ℕ) :=
   Nat.Primrec.comp .succ CompatibleEncodingRelation.decode_primrec
 
-def Encoding.of {α_base : Type u} {α : new_type% α_base}
-    [Encodable α_base] [CompatibleEncodingRelation α]
-    (x : α_base) : Encoding α := ⟨CompatibleEncodingRelation.decode α (Encodable.encode x)⟩
+def Encoding.of {α : Type u} {α_extra : new_type% α}
+    [Encodable α] [CompatibleEncodingRelation α_extra]
+    (x : α) : Encoding α_extra := ⟨CompatibleEncodingRelation.decode α_extra (Encodable.encode x)⟩
 
-theorem Encoding.encode_of {α_base : Type u} {α : new_type% α_base}
-    [Encodable α_base] [CompatibleEncodingRelation α]
-    (x : α_base) : Encodable.encode (Encoding.of (α := α) x) = Encodable.encode x := by
-  obtain ⟨n, hn⟩ := FullyRepresentable.isRepresentable (InhabitedExtra.default x : α.1 x)
+theorem Encoding.encode_of {α : Type u} {α_extra : new_type% α}
+    [Encodable α] [CompatibleEncodingRelation α_extra]
+    (x : α) : Encodable.encode (Encoding.of (α_extra := α_extra) x) = Encodable.encode x := by
+  obtain ⟨n, hn⟩ := FullyRepresentable.isRepresentable (InhabitedExtra.default x : α_extra.1 x)
   simp [of, ← Encoding.encode_eq hn, Encodable.encode]
 
-theorem Encoding.encoding_of {α_base : Type u} {α : new_type% α_base}
-    [Encodable α_base] [CompatibleEncodingRelation α]
-    {x_base : α_base} (x : new_type% x_base) :
-    α.2 x (Encoding.of (α := α) x_base).repr := by
-  obtain ⟨n, hn⟩ := FullyRepresentable.isRepresentable x
+theorem Encoding.encoding_of {α : Type u} {α_extra : new_type% α}
+    [Encodable α] [CompatibleEncodingRelation α_extra]
+    {x : α} (x_extra : new_type% x) :
+    α_extra.2 x_extra (Encoding.of (α_extra := α_extra) x).repr := by
+  obtain ⟨n, hn⟩ := FullyRepresentable.isRepresentable x_extra
   simp [of, ← Encoding.encode_eq hn, Encodable.encode, hn]
 
 open CompatibleEncodingRelation in
-theorem Encoding.primrec_of {α_base : Type u} {α : new_type% α_base}
-    [Primcodable α_base] [CompatibleEncodingRelation α] :
-    Primrec (Encoding.of : α_base → Encoding α) := by
+theorem Encoding.primrec_of {α : Type u} {α_extra : new_type% α}
+    [Primcodable α] [CompatibleEncodingRelation α_extra] :
+    Primrec (Encoding.of : α → Encoding α_extra) := by
   unfold of
   exact .comp primrec_mk (.comp (Primrec.nat_iff.mpr decode_primrec) .encode)
 
-theorem dprimrec_iff_primrec {α_base : Type u} {α : new_type% α_base}
-    {β_base : Type v} {β : new_type% β_base} [Primcodable α_base] [Primcodable β_base]
-    [CompatibleEncodingRelation α] [CompatibleEncodingRelation β]
-    {f_base : α_base → β_base} (f : new_type% f_base) :
-    DPrimrec f ↔ Primrec f_base := by
+theorem dprimrec_iff_primrec {α : Type u} {α_extra : new_type% α}
+    {β : Type v} {β_extra : new_type% β} [Primcodable α] [Primcodable β]
+    [CompatibleEncodingRelation α_extra] [CompatibleEncodingRelation β_extra]
+    {f : α → β} (f_extra : new_type% f) :
+    DPrimrec f_extra ↔ Primrec f := by
   constructor
   · rintro ⟨g, hgprim, hg'⟩
     rw [Primrec]
     rw [← Primrec.nat_iff] at hgprim ⊢
-    let g' (a : Encoding α) : Encoding β := ⟨g a.repr⟩
-    have commute (a : α_base) : g' (Encoding.of a) = Encoding.of (f_base a) := by
-      have := hg' (Encoding.encoding_of (InhabitedExtra.default a : α.1 a))
+    let g' (a : Encoding α_extra) : Encoding β_extra := ⟨g a.repr⟩
+    have commute (a : α) : g' (Encoding.of a) = Encoding.of (f a) := by
+      have := hg' (Encoding.encoding_of (InhabitedExtra.default a : α_extra.1 a))
       simp [Encoding.of, g', ← Encoding.encode_eq this, Encodable.encode]
     have hg'prim : Primrec g' := .comp Encoding.primrec_mk (.comp hgprim Encoding.primrec_repr)
     let fn (n : ℕ) : ℕ :=
-      (Encodable.decode n : Option α_base).casesOn 0
+      (Encodable.decode n : Option α).casesOn 0
         (fun a => Encodable.encode (g' (Encoding.of a)) + 1)
     have : Primrec fn :=
       .option_casesOn .decode (.const 0)
@@ -493,33 +496,33 @@ theorem dprimrec_iff_primrec {α_base : Type u} {α : new_type% α_base}
     refine this.of_eq ?_
     intro n
     simp only [fn]
-    rcases h : (Encodable.decode n : Option α_base) with _ | a
+    rcases h : (Encodable.decode n : Option α) with _ | a
     · simp
-    · have := Encoding.encode_of (α := β) (f_base a)
+    · have := Encoding.encode_of (α_extra := β_extra) (f a)
       simp [← this, commute]
   · intro hf
     let fn (n : ℕ) : ℕ :=
-      (Encodable.decode (Encodable.encode (⟨n⟩ : Encoding α)) : Option α_base).casesOn
-        0 (fun a => (Encoding.of (α := β) (f_base a)).repr)
+      (Encodable.decode (Encodable.encode (⟨n⟩ : Encoding α_extra)) : Option α).casesOn
+        0 (fun a => (Encoding.of (α_extra := β_extra) (f a)).repr)
     refine ⟨fn, ?_, ?_⟩
     · rw [← Primrec.nat_iff]
       exact .option_casesOn (.comp .decode (.comp .encode Encoding.primrec_mk)) (.const 0) <|
         Encoding.primrec_repr.comp (Encoding.primrec_of.comp (hf.comp .snd))
-    · intro a_base a n han
+    · intro a a n han
       simp [fn, Encoding.encode_eq han, Encoding.encoding_of]
 
-theorem dcomputable_iff_computable {α_base : Type u} {α : new_type% α_base}
-    {β_base : Type v} {β : new_type% β_base} [Primcodable α_base] [Primcodable β_base]
-    [CompatibleEncodingRelation α] [CompatibleEncodingRelation β]
-    {f_base : α_base → β_base} (f : new_type% f_base) :
-    DComputable f ↔ Computable f_base := by
+theorem dcomputable_iff_computable {α : Type u} {α_extra : new_type% α}
+    {β : Type v} {β_extra : new_type% β} [Primcodable α] [Primcodable β]
+    [CompatibleEncodingRelation α_extra] [CompatibleEncodingRelation β_extra]
+    {f : α → β} (f_extra : new_type% f) :
+    DComputable f_extra ↔ Computable f := by
   constructor
   · rintro ⟨g, hgprim, hg'⟩
     rw [Computable, Partrec]
     rw [← Partrec.nat_iff] at hgprim ⊢
-    let g' (a : Encoding α) : Part (Encoding β) := (g a.repr).map Encoding.mk
-    have commute (a : α_base) : g' (Encoding.of a) = Part.some (Encoding.of (f_base a)) := by
-      obtain ⟨y, hy, this⟩ := hg' (Encoding.encoding_of (InhabitedExtra.default a : α.1 a))
+    let g' (a : Encoding α_extra) : Part (Encoding β_extra) := (g a.repr).map Encoding.mk
+    have commute (a : α) : g' (Encoding.of a) = Part.some (Encoding.of (f a)) := by
+      obtain ⟨y, hy, this⟩ := hg' (Encoding.encoding_of (InhabitedExtra.default a : α_extra.1 a))
       simp only [Encoding.of] at hy
       simp [Encoding.of, g', ← Encoding.encode_eq this, Part.eq_some_iff.mpr hy, Encodable.encode]
     have hg'part : Partrec g' :=
@@ -534,14 +537,14 @@ theorem dcomputable_iff_computable {α_base : Type u} {α : new_type% α_base}
     refine this.of_eq ?_
     intro n
     simp only [fn]
-    rcases h : (Encodable.decode n : Option α_base) with _ | a
+    rcases h : (Encodable.decode n : Option α) with _ | a
     · simp
-    · have := Encoding.encode_of (α := β) (f_base a)
+    · have := Encoding.encode_of (α_extra := β_extra) (f a)
       simp [← this, commute]
   · intro hf
     let fn (n : ℕ) : ℕ :=
-      (Encodable.decode (Encodable.encode (⟨n⟩ : Encoding α)) : Option α_base).casesOn
-        0 (fun a => (Encoding.of (α := β) (f_base a)).repr)
+      (Encodable.decode (Encodable.encode (⟨n⟩ : Encoding α_extra)) : Option α).casesOn
+        0 (fun a => (Encoding.of (α_extra := β_extra) (f a)).repr)
     refine ⟨fn, ?_, ?_⟩
     · rw [← Partrec.nat_iff]
       change Computable fn
@@ -549,161 +552,161 @@ theorem dcomputable_iff_computable {α_base : Type u} {α : new_type% α_base}
       exact .option_casesOn (.comp .decode (.comp .encode Encoding.primrec_mk.to_comp))
         (.const 0) (Encoding.primrec_repr.to_comp.comp (Encoding.primrec_of.to_comp.comp
           (hf.comp .snd)))
-    · intro a_base a n han
+    · intro a a n han
       simp [fn, Encoding.encode_eq han, Encoding.encoding_of]
 
-protected theorem DPrimrec.id {α_base : Sort u} {α : new_type% α_base} :
-    DPrimrec (fun ⦃a_base : α_base⦄ (a : α.1 a_base) => a) := by
+protected theorem DPrimrec.id {α : Sort u} {α_extra : new_type% α} :
+    DPrimrec (fun ⦃a : α⦄ (a : α_extra.1 a) => a) := by
   use id, .id
   simp
 
-protected theorem DPrimrec.const' {α_base : Sort u} {α : new_type% α_base}
-    {β_base : Sort v} {β : new_type% β_base}
-    {x_base : β_base} {x : new_type% x_base}
-    (h : IsRepresentable x) :
-    DPrimrec (fun ⦃a_base : α_base⦄ (_ : α.1 a_base) => x) := by
+protected theorem DPrimrec.const' {α : Sort u} {α_extra : new_type% α}
+    {β : Sort v} {β_extra : new_type% β}
+    {x : β} {x_extra : new_type% x}
+    (h : IsRepresentable x_extra) :
+    DPrimrec (fun ⦃a : α⦄ (_ : α_extra.1 a) => x_extra) := by
   obtain ⟨n, hn⟩ := h
   use fun _ => n, .const n
-  intro a_base a b hab
+  intro a a b hab
   assumption
 
-protected theorem DPrimrec.const {α_base : Sort u} {α : new_type% α_base}
-    {β_base : Sort v} {β : new_type% β_base}
-    [FullyRepresentable β] {x_base : β_base} (x : β.1 x_base) :
-    DPrimrec (fun ⦃a_base : α_base⦄ (_ : α.1 a_base) => x) :=
+protected theorem DPrimrec.const {α : Sort u} {α_extra : new_type% α}
+    {β : Sort v} {β_extra : new_type% β}
+    [FullyRepresentable β_extra] {x : β} (x : β_extra.1 x) :
+    DPrimrec (fun ⦃a : α⦄ (_ : α_extra.1 a) => x) :=
   .const' (FullyRepresentable.isRepresentable x)
 
 protected theorem DPrimrec.comp.{u}
-    {β_base : Sort v} {β : new_type% β_base}
-    {γ_base : β_base → Sort w} {γ : new_type% γ_base}
-    {f_base : (x : β_base) → γ_base x} {f : new_type% f_base}
-    (hf : DPrimrec f)
-    {α_base : Sort u} {α : new_type% α_base}
-    {g_base : α_base → β_base} {g : new_type% g_base}
-    (hg : DPrimrec g) :
-    DPrimrec (new% (fun a => f_base (g_base a))) := by
+    {β : Sort v} {β_extra : new_type% β}
+    {γ : β → Sort w} {γ_extra : new_type% γ}
+    {f : (x : β) → γ x} {f_extra : new_type% f}
+    (hf : DPrimrec f_extra)
+    {α : Sort u} {α_extra : new_type% α}
+    {g : α → β} {g_extra : new_type% g}
+    (hg : DPrimrec g_extra) :
+    DPrimrec (new% (fun a => f (g a))) := by
   obtain ⟨gf, hgf, hgf'⟩ := hf
   obtain ⟨gg, hgg, hgg'⟩ := hg
   refine ⟨_, hgf.comp hgg, ?_⟩
-  intro a_base a b hab
+  intro a a b hab
   exact hgf' (hgg' hab)
 
-protected theorem DPrimrec.of_isProp {α_base : Sort u} {α : new_type% α_base}
-    {β_base : α_base → Sort v} {β : new_type% β_base}
-    {f_base : (a : α_base) → β_base a} {f : new_type% f_base}
+protected theorem DPrimrec.of_isProp {α : Sort u} {α_extra : new_type% α}
+    {β : α → Sort v} {β_extra : new_type% β}
+    {f : (a : α) → β a} {f_extra : new_type% f}
     (hprop : IsProp.{v}) :
-    DPrimrec f := by
+    DPrimrec f_extra := by
   use fun _ => 0, .zero
-  intro a_base a n h
-  exact ((β a).3 hprop (f a) 0).mpr .zero
+  intro a a n h
+  exact ((β_extra a).3 hprop (f_extra a) 0).mpr .zero
 
-protected theorem DPrimrec.proof {α_base : Sort u} {α : new_type% α_base}
-    {β_base : α_base → Prop} {β : new_type% β_base}
-    {f_base : (a : α_base) → β_base a} {f : new_type% f_base} :
-    DPrimrec f := .of_isProp isProp_prop
+protected theorem DPrimrec.proof {α : Sort u} {α_extra : new_type% α}
+    {β : α → Prop} {β_extra : new_type% β}
+    {f : (a : α) → β a} {f_extra : new_type% f} :
+    DPrimrec f_extra := .of_isProp isProp_prop
 
 protected theorem DPrimrec.irrelevant
-    {α_base : Sort u} {α : new_type% α_base}
-    {β_base : α_base → Sort v} {β : new_type% β_base}
-    [∀ ⦃a_base⦄ (a : α.1 a_base), Irrelevant (β a)]
-    {f_base : (a : α_base) → β_base a} {f : new_type% f_base} :
-    DPrimrec (new% f_base) := by
+    {α : Sort u} {α_extra : new_type% α}
+    {β : α → Sort v} {β_extra : new_type% β}
+    [∀ ⦃a⦄ (a : α_extra.1 a), Irrelevant (β_extra a)]
+    {f : (a : α) → β a} {f_extra : new_type% f} :
+    DPrimrec (new% f) := by
   use fun _ => 0, .zero
   simp [Irrelevant.encoding]
 
-protected theorem DPrimrec.sort {α_base : Sort u} {α : new_type% α_base}
-    {f_base : α_base → Sort v} {f : new_type% f_base} :
-    DPrimrec (new% f_base) := .irrelevant
+protected theorem DPrimrec.sort {α : Sort u} {α_extra : new_type% α}
+    {f : α → Sort v} {f_extra : new_type% f} :
+    DPrimrec (new% f) := .irrelevant
 
 protected theorem DPrimrec.dcomputable
-    {α_base : Sort u} {α : new_type% α_base}
-    {β_base : α_base → Sort v} {β : new_type% β_base}
-    {f_base : (a : α_base) → β_base a} {f : new_type% f_base}
-    (hf : DPrimrec f) : DComputable f := by
+    {α : Sort u} {α_extra : new_type% α}
+    {β : α → Sort v} {β_extra : new_type% β}
+    {f : (a : α) → β a} {f_extra : new_type% f}
+    (hf : DPrimrec f_extra) : DComputable f_extra := by
   obtain ⟨g, hg, hg'⟩ := hf
   use g, .of_primrec hg
-  intro a_base a n h
+  intro a a n h
   use g n
   simpa using hg' h
 
 alias DComputable.of_prim := DPrimrec.dcomputable
 
-protected theorem DComputable.id {α_base : Sort u} {α : new_type% α_base} :
-    DComputable (fun ⦃a_base : α_base⦄ (a : α.1 a_base) => a) := .of_prim .id
+protected theorem DComputable.id {α : Sort u} {α_extra : new_type% α} :
+    DComputable (fun ⦃a : α⦄ (a : α_extra.1 a) => a) := .of_prim .id
 
-protected theorem DComputable.const' {α_base : Sort u} {α : new_type% α_base}
-    {β_base : Sort v} {β : new_type% β_base}
-    {x_base : β_base} {x : new_type% x_base}
-    (h : IsRepresentable x) :
-    DComputable (fun ⦃a_base : α_base⦄ (_ : α.1 a_base) => x) := .of_prim (.const' h)
+protected theorem DComputable.const' {α : Sort u} {α_extra : new_type% α}
+    {β : Sort v} {β_extra : new_type% β}
+    {x : β} {x_extra : new_type% x}
+    (h : IsRepresentable x_extra) :
+    DComputable (fun ⦃a : α⦄ (_ : α_extra.1 a) => x_extra) := .of_prim (.const' h)
 
-protected theorem DComputable.const {α_base : Sort u} {α : new_type% α_base}
-    {β_base : Sort v} {β : new_type% β_base}
-    [FullyRepresentable β] {x_base : β_base} {x : new_type% x_base} :
-    DComputable (fun ⦃a_base : α_base⦄ (_ : α.1 a_base) => x) := .of_prim (.const x)
+protected theorem DComputable.const {α : Sort u} {α_extra : new_type% α}
+    {β : Sort v} {β_extra : new_type% β}
+    [FullyRepresentable β_extra] {x : β} {x_extra : new_type% x} :
+    DComputable (fun ⦃a : α⦄ (_ : α_extra.1 a) => x_extra) := .of_prim (.const x_extra)
 
 protected theorem DComputable.comp.{u}
-    {β_base : Sort v} {β : new_type% β_base}
-    {γ_base : β_base → Sort w} {γ : new_type% γ_base}
-    {f_base : (x : β_base) → γ_base x} {f : new_type% f_base}
-    (hf : DComputable f)
-    {α_base : Sort u} {α : new_type% α_base}
-    {g_base : α_base → β_base} {g : new_type% g_base}
-    (hg : DComputable g) :
-    DComputable (new% (fun a => f_base (g_base a))) := by
+    {β : Sort v} {β_extra : new_type% β}
+    {γ : β → Sort w} {γ_extra : new_type% γ}
+    {f : (x : β) → γ x} {f_extra : new_type% f}
+    (hf : DComputable f_extra)
+    {α : Sort u} {α_extra : new_type% α}
+    {g : α → β} {g_extra : new_type% g}
+    (hg : DComputable g_extra) :
+    DComputable (new% (fun a => f (g a))) := by
   obtain ⟨gf, hgf, hgf'⟩ := hf
   obtain ⟨gg, hgg, hgg'⟩ := hg
   refine ⟨_, hgf.comp hgg, ?_⟩
-  intro a_base a n han
+  intro a a n han
   obtain ⟨x, hx, hx'⟩ := hgg' han
   obtain ⟨y, hy, hy'⟩ := hgf' hx'
   simp only [Part.bind_eq_bind, Part.mem_bind_iff]
   exact ⟨y, ⟨x, hx, hy⟩, hy'⟩
 
 protected theorem DPrimrec.compComputable.{u}
-    {β_base : Sort v} {β : new_type% β_base}
-    {γ_base : β_base → Sort w} {γ : new_type% γ_base}
-    {f_base : (x : β_base) → γ_base x} {f : new_type% f_base}
-    (hf : DPrimrec f)
-    {α_base : Sort u} {α : new_type% α_base}
-    {g_base : α_base → β_base} {g : new_type% g_base}
-    (hg : DComputable g) :
-    DComputable (new% (fun a => f_base (g_base a))) :=
+    {β : Sort v} {β_extra : new_type% β}
+    {γ : β → Sort w} {γ_extra : new_type% γ}
+    {f : (x : β) → γ x} {f_extra : new_type% f}
+    (hf : DPrimrec f_extra)
+    {α : Sort u} {α_extra : new_type% α}
+    {g : α → β} {g_extra : new_type% g}
+    (hg : DComputable g_extra) :
+    DComputable (new% (fun a => f (g a))) :=
   .comp (.of_prim hf) hg
 
-protected theorem DComputable.of_isProp {α_base : Sort u} {α : new_type% α_base}
-    {β_base : α_base → Sort v} {β : new_type% β_base}
-    {f_base : (a : α_base) → β_base a} {f : new_type% f_base}
+protected theorem DComputable.of_isProp {α : Sort u} {α_extra : new_type% α}
+    {β : α → Sort v} {β_extra : new_type% β}
+    {f : (a : α) → β a} {f_extra : new_type% f}
     (hprop : IsProp.{v}) :
-    DComputable f := .of_prim (.of_isProp hprop)
+    DComputable f_extra := .of_prim (.of_isProp hprop)
 
-protected theorem DComputable.proof {α_base : Sort u} {α : new_type% α_base}
-    {β_base : α_base → Prop} {β : new_type% β_base}
-    {f_base : (a : α_base) → β_base a} {f : new_type% f_base} :
-    DComputable f := .of_prim .proof
+protected theorem DComputable.proof {α : Sort u} {α_extra : new_type% α}
+    {β : α → Prop} {β_extra : new_type% β}
+    {f : (a : α) → β a} {f_extra : new_type% f} :
+    DComputable f_extra := .of_prim .proof
 
 protected theorem DComputable.irrelevant
-    {α_base : Sort u} {α : new_type% α_base}
-    {β_base : α_base → Sort v} {β : new_type% β_base}
-    [∀ ⦃a_base⦄ (a : α.1 a_base), Irrelevant (β a)]
-    {f_base : (a : α_base) → β_base a} {f : new_type% f_base} :
-    DComputable (new% f_base) := .of_prim .irrelevant
+    {α : Sort u} {α_extra : new_type% α}
+    {β : α → Sort v} {β_extra : new_type% β}
+    [∀ ⦃a⦄ (a : α_extra.1 a), Irrelevant (β_extra a)]
+    {f : (a : α) → β a} {f_extra : new_type% f} :
+    DComputable (new% f) := .of_prim .irrelevant
 
-protected theorem DComputable.sort {α_base : Sort u} {α : new_type% α_base}
-    {f_base : α_base → Sort v} {f : new_type% f_base} :
-    DComputable (new% f_base) := .of_prim .sort
+protected theorem DComputable.sort {α : Sort u} {α_extra : new_type% α}
+    {f : α → Sort v} {f_extra : new_type% f} :
+    DComputable (new% f) := .of_prim .sort
 
-inductive New.PSigma._induct {α_base : Sort u} {α : new_type% α_base}
-    {β_base : α_base → Sort v} (β : new_type% β_base)
-    (p_base : PSigma β_base) : Sort (max 1 u v) where
-  | mk (fst : α.1 p_base.1) (snd : (β fst).1 p_base.2)
+inductive New.PSigma._induct {α : Sort u} {α_extra : new_type% α}
+    {β : α → Sort v} (β_extra : new_type% β)
+    (p : PSigma β) : Sort (max 1 u v) where
+  | mk (fst : α_extra.1 p.1) (snd : (β_extra fst).1 p.2)
 
-inductive New.PSigma._encoding {α_base : Sort u} {α : new_type% α_base}
-    {β_base : α_base → Sort v} (β : new_type% β_base)
-    ⦃p_base : PSigma β_base⦄ (p : New.PSigma._induct β p_base) :
+inductive New.PSigma._encoding {α : Sort u} {α_extra : new_type% α}
+    {β : α → Sort v} (β_extra : new_type% β)
+    ⦃p : PSigma β⦄ (p : New.PSigma._induct β_extra p) :
     (n : ℕ) → Prop where
-  | mk {fst_n : ℕ} (fst : α.2 p.1 fst_n) {snd_n : ℕ} (snd : (β _).2 p.2 snd_n) :
-    _encoding β p (Nat.pair fst_n snd_n)
+  | mk {fst_n : ℕ} (fst : α_extra.2 p.1 fst_n) {snd_n : ℕ} (snd : (β_extra _).2 p.2 snd_n) :
+    _encoding β_extra p (Nat.pair fst_n snd_n)
 
 def New.PSigma.{u, v} : new_type% @PSigma.{u, v} := fun _ _ _ β =>
   .mk (New.PSigma._induct β) (New.PSigma._encoding β) not_isProp.{max u v}.elim
@@ -721,15 +724,15 @@ def New.PSigma.rec.{u_1, u, v} : new_type% @PSigma.rec.{u_1, u, v} :=
   fun _ _ _ _ _ _ _ mk _ t => mk t.1 t.2
 
 theorem New.PSigma.mk.primrec.{c, u, v}
-    {ctx_base : Sort c} {ctx : new_type% ctx_base}
-    {α_base : ctx_base → Sort u} {α : new_type% α_base}
-    {β_base : (c : ctx_base) → α_base c → Sort v} {β : new_type% β_base}
-    {fst_base : (c : ctx_base) → α_base c} {fst : new_type% fst_base}
-    (fst_prim : DPrimrec fst)
-    {snd_base : (c : ctx_base) → β_base c (fst_base c)} {snd : new_type% snd_base}
-    (snd_prim : DPrimrec snd) :
+    {ctx : Sort c} {ctx_extra : new_type% ctx}
+    {α : ctx → Sort u} {α_extra : new_type% α}
+    {β : (c : ctx) → α c → Sort v} {β_extra : new_type% β}
+    {fst : (c : ctx) → α c} {fst_extra : new_type% fst}
+    (fst_prim : DPrimrec fst_extra)
+    {snd : (c : ctx) → β c (fst c)} {snd_extra : new_type% snd}
+    (snd_prim : DPrimrec snd_extra) :
     DPrimrec (new% fun c =>
-      @_root_.PSigma.mk (α_base c) (β_base c) (fst_base c) (snd_base c)) := by
+      @_root_.PSigma.mk (α c) (β c) (fst c) (snd c)) := by
   obtain ⟨f, hf, hf'⟩ := fst_prim
   obtain ⟨g, hg, hg'⟩ := snd_prim
   refine ⟨_, .pair hf hg, ?_⟩
@@ -741,51 +744,51 @@ theorem New.PSigma.mk.primrec.{c, u, v}
     assumption
 
 theorem New.PSigma.fst.primrec.{c, u, v}
-    {ctx_base : Sort c} {ctx : new_type% ctx_base}
-    {α_base : ctx_base → Sort u} {α : new_type% α_base}
-    {β_base : (c : ctx_base) → α_base c → Sort v} {β : new_type% β_base}
-    {self_base : (c : ctx_base) → (a : α_base c) ×' β_base c a}
-    {self : new_type% self_base}
-    (self_prim : DPrimrec (new% self_base)) :
+    {ctx : Sort c} {ctx_extra : new_type% ctx}
+    {α : ctx → Sort u} {α_extra : new_type% α}
+    {β : (c : ctx) → α c → Sort v} {β_extra : new_type% β}
+    {self : (c : ctx) → (a : α c) ×' β c a}
+    {self_extra : new_type% self}
+    (self_prim : DPrimrec (new% self)) :
     DPrimrec (new% fun c =>
-      @_root_.PSigma.fst (α_base c) (β_base c) (self_base c)) := by
+      @_root_.PSigma.fst (α c) (β c) (self c)) := by
   obtain ⟨f, hf, hf'⟩ := self_prim
   refine ⟨_, .comp .left hf, ?_⟩
-  intro a_base a n han
+  intro a a n han
   refine (hf' han).casesOn ?_
   intros
   simpa
 
 theorem New.PSigma.snd.primrec.{c, u, v}
-    {ctx_base : Sort c} {ctx : new_type% ctx_base}
-    {α_base : ctx_base → Sort u} {α : new_type% α_base}
-    {β_base : (c : ctx_base) → α_base c → Sort v} {β : new_type% β_base}
-    {self_base : (c : ctx_base) → (a : α_base c) ×' β_base c a}
-    {self : new_type% self_base}
-    (self_prim : DPrimrec (new% self_base)) :
+    {ctx : Sort c} {ctx_extra : new_type% ctx}
+    {α : ctx → Sort u} {α_extra : new_type% α}
+    {β : (c : ctx) → α c → Sort v} {β_extra : new_type% β}
+    {self : (c : ctx) → (a : α c) ×' β c a}
+    {self_extra : new_type% self}
+    (self_prim : DPrimrec (new% self)) :
     DPrimrec (new% fun c =>
-      @_root_.PSigma.snd (α_base c) (β_base c) (self_base c)) := by
+      @_root_.PSigma.snd (α c) (β c) (self c)) := by
   obtain ⟨f, hf, hf'⟩ := self_prim
   refine ⟨_, .comp .right hf, ?_⟩
-  intro a_base a n han
+  intro a a n han
   refine (hf' han).casesOn ?_
   intros
   simpa
 
 theorem New.PSigma.mk.computable.{c, u, v}
-    {ctx_base : Sort c} {ctx : new_type% ctx_base}
-    {α_base : ctx_base → Sort u} {α : new_type% α_base}
-    {β_base : (c : ctx_base) → α_base c → Sort v} {β : new_type% β_base}
-    {fst_base : (c : ctx_base) → α_base c} {fst : new_type% fst_base}
-    (fst_prim : DComputable fst)
-    {snd_base : (c : ctx_base) → β_base c (fst_base c)} {snd : new_type% snd_base}
-    (snd_prim : DComputable snd) :
+    {ctx : Sort c} {ctx_extra : new_type% ctx}
+    {α : ctx → Sort u} {α_extra : new_type% α}
+    {β : (c : ctx) → α c → Sort v} {β_extra : new_type% β}
+    {fst : (c : ctx) → α c} {fst_extra : new_type% fst}
+    (fst_prim : DComputable fst_extra)
+    {snd : (c : ctx) → β c (fst c)} {snd_extra : new_type% snd}
+    (snd_prim : DComputable snd_extra) :
     DComputable (new% fun c =>
-      @_root_.PSigma.mk (α_base c) (β_base c) (fst_base c) (snd_base c)) := by
+      @_root_.PSigma.mk (α c) (β c) (fst c) (snd c)) := by
   obtain ⟨f, hf, hf'⟩ := fst_prim
   obtain ⟨g, hg, hg'⟩ := snd_prim
   refine ⟨_, .pair hf hg, ?_⟩
-  intro a_base a n han
+  intro a a n han
   obtain ⟨n₁, hn₁, hn₁'⟩ := hf' han
   obtain ⟨n₂, hn₂, hn₂'⟩ := hg' han
   use Nat.pair n₁ n₂
@@ -794,34 +797,34 @@ theorem New.PSigma.mk.computable.{c, u, v}
   constructor <;> simpa
 
 theorem New.PSigma.fst.computable.{c, u, v}
-    {ctx_base : Sort c} {ctx : new_type% ctx_base}
-    {α_base : ctx_base → Sort u} {α : new_type% α_base}
-    {β_base : (c : ctx_base) → α_base c → Sort v} {β : new_type% β_base}
-    {self_base : (c : ctx_base) → (a : α_base c) ×' β_base c a}
-    {self : new_type% self_base}
-    (self_prim : DComputable (new% self_base)) :
+    {ctx : Sort c} {ctx_extra : new_type% ctx}
+    {α : ctx → Sort u} {α_extra : new_type% α}
+    {β : (c : ctx) → α c → Sort v} {β_extra : new_type% β}
+    {self : (c : ctx) → (a : α c) ×' β c a}
+    {self_extra : new_type% self}
+    (self_prim : DComputable (new% self)) :
     DComputable (new% fun c =>
-      @_root_.PSigma.fst (α_base c) (β_base c) (self_base c)) := by
+      @_root_.PSigma.fst (α c) (β c) (self c)) := by
   obtain ⟨f, hf, hf'⟩ := self_prim
   refine ⟨_, .comp .left hf, ?_⟩
-  intro a_base a n han
+  intro a a n han
   simp only [Part.bind_eq_bind, Part.mem_bind_iff, PFun.coe_val, Part.mem_some_iff, ↓existsAndEq,
     and_true]
   obtain @⟨_, hy, x, hy₁, x', hy₂⟩ := hf' han
   exact ⟨_, hy, by simpa using hy₁⟩
 
 theorem New.PSigma.snd.computable.{c, u, v}
-    {ctx_base : Sort c} {ctx : new_type% ctx_base}
-    {α_base : ctx_base → Sort u} {α : new_type% α_base}
-    {β_base : (c : ctx_base) → α_base c → Sort v} {β : new_type% β_base}
-    {self_base : (c : ctx_base) → (a : α_base c) ×' β_base c a}
-    {self : new_type% self_base}
-    (self_prim : DComputable (new% self_base)) :
+    {ctx : Sort c} {ctx_extra : new_type% ctx}
+    {α : ctx → Sort u} {α_extra : new_type% α}
+    {β : (c : ctx) → α c → Sort v} {β_extra : new_type% β}
+    {self : (c : ctx) → (a : α c) ×' β c a}
+    {self_extra : new_type% self}
+    (self_prim : DComputable (new% self)) :
     DComputable (new% fun c =>
-      @_root_.PSigma.snd (α_base c) (β_base c) (self_base c)) := by
+      @_root_.PSigma.snd (α c) (β c) (self c)) := by
   obtain ⟨f, hf, hf'⟩ := self_prim
   refine ⟨_, .comp .right hf, ?_⟩
-  intro a_base a n han
+  intro a a n han
   simp only [Part.bind_eq_bind, Part.mem_bind_iff, PFun.coe_val, Part.mem_some_iff, ↓existsAndEq,
     and_true]
   obtain @⟨_, hy, x, hy₁, x', hy₂⟩ := hf' han
@@ -829,12 +832,12 @@ theorem New.PSigma.snd.computable.{c, u, v}
 
 open Nat.Partrec (Code) in
 theorem DPrimrec.curry
-    {α_base : Sort u} {α : new_type% α_base}
-    {β_base : α_base → Sort v} {β : new_type% β_base}
-    {γ_base : (a : α_base) → β_base a → Sort w} {γ : new_type% γ_base}
-    {f_base : (a : α_base) → (b : β_base a) → γ_base a b} {f : new_type% f_base}
-    (hf : DComputable (new% fun x : (a : α_base) ×' β_base a => f_base x.1 x.2)) :
-    DPrimrec (new% f_base) := by
+    {α : Sort u} {α_extra : new_type% α}
+    {β : α → Sort v} {β_extra : new_type% β}
+    {γ : (a : α) → β a → Sort w} {γ_extra : new_type% γ}
+    {f : (a : α) → (b : β a) → γ a b} {f_extra : new_type% f}
+    (hf : DComputable (new% fun x : (a : α) ×' β a => f x.1 x.2)) :
+    DPrimrec (new% f) := by
   by_cases hprop : IsProp.{imax v w}
   · exact .of_isProp hprop
   obtain ⟨g, hg, hc⟩ := hf
@@ -843,73 +846,73 @@ theorem DPrimrec.curry
     rw [← Primrec.nat_iff]
     exact .comp .encode (Code.primrec₂_curry.comp (.const c) .id)
   refine ⟨_, this, ?_⟩
-  intro a_base a n hna
+  intro a a n hna
   rw [encoding_pi_def hprop]
-  intro b_base b m hmb
+  intro b b m hmb
   simp only [Denumerable.ofNat_encode, Code.eval_curry]
   exact @hc ⟨_, _⟩ ⟨a, b⟩ (Nat.pair n m) ⟨by simpa, by simpa⟩
 
 theorem DPrimrec.constCurry.{u}
-    {β_base : Sort v} {β : new_type% β_base}
-    {γ_base : β_base → Sort w} {γ : new_type% γ_base}
-    {f_base : (a : β_base) → γ_base a} {f : new_type% f_base}
-    (hf : DComputable f)
-    {α_base : Sort u} {α : new_type% α_base} :
-    DPrimrec (new% fun _ : α_base => f_base) := by
-  refine .const' (x := new% f_base) ?_
+    {β : Sort v} {β_extra : new_type% β}
+    {γ : β → Sort w} {γ_extra : new_type% γ}
+    {f : (a : β) → γ a} {f_extra : new_type% f}
+    (hf : DComputable f_extra)
+    {α : Sort u} {α_extra : new_type% α} :
+    DPrimrec (new% fun _ : α => f) := by
+  refine .const' (x_extra := new% f) ?_
   rwa [isRepresentable_function_iff]
 
 protected theorem DComputable.constCurry.{u}
-    {β_base : Sort v} {β : new_type% β_base}
-    {γ_base : β_base → Sort w} {γ : new_type% γ_base}
-    {f_base : (a : β_base) → γ_base a} {f : new_type% f_base}
-    (hf : DComputable f)
-    {α_base : Sort u} {α : new_type% α_base} :
-    DComputable (new% fun _ : α_base => f_base) :=
+    {β : Sort v} {β_extra : new_type% β}
+    {γ : β → Sort w} {γ_extra : new_type% γ}
+    {f : (a : β) → γ a} {f_extra : new_type% f}
+    (hf : DComputable f_extra)
+    {α : Sort u} {α_extra : new_type% α} :
+    DComputable (new% fun _ : α => f) :=
   .of_prim (.constCurry hf)
 
 theorem DPrimrec.curriedApp.{u}
-    {α_base : Sort u} {α : new_type% α_base}
-    {β_base : α_base → Sort v} {β : new_type% β_base}
-    {γ_base : (a : α_base) → β_base a → Sort w} {γ : new_type% γ_base}
-    {f_base : (a : α_base) → (b : β_base a) → γ_base a b} {f : new_type% f_base}
-    (hf : DPrimrec (new% fun x : (a : α_base) ×' β_base a => f_base x.1 x.2))
-    {g_base : (a : α_base) → β_base a} {g : new_type% g_base}
-    (hg : DPrimrec g) :
-    DPrimrec (new% fun x => f_base x (g_base x)) :=
+    {α : Sort u} {α_extra : new_type% α}
+    {β : α → Sort v} {β_extra : new_type% β}
+    {γ : (a : α) → β a → Sort w} {γ_extra : new_type% γ}
+    {f : (a : α) → (b : β a) → γ a b} {f_extra : new_type% f}
+    (hf : DPrimrec (new% fun x : (a : α) ×' β a => f x.1 x.2))
+    {g : (a : α) → β a} {g_extra : new_type% g}
+    (hg : DPrimrec g_extra) :
+    DPrimrec (new% fun x => f x (g x)) :=
   .comp hf (New.PSigma.mk.primrec .id hg)
 
 example
-    {β_base : Sort v} {β : new_type% β_base}
-    {γ_base : β_base → Sort w} {γ : new_type% γ_base}
-    {δ_base : (a : β_base) → γ_base a → Sort w'} {δ : new_type% δ_base}
-    {f_base : (a : β_base) → (b : γ_base a) → δ_base a b} {f : new_type% f_base}
-    (hf : DPrimrec (new% fun x : (a : β_base) ×' γ_base a => f_base x.1 x.2))
-    {α_base : Sort u} {α : new_type% α_base}
-    {g₁_base : α_base → β_base} {g₁ : new_type% g₁_base}
-    (hg₁ : DPrimrec g₁)
-    {g₂_base : (a : α_base) → γ_base (g₁_base a)} {g₂ : new_type% g₂_base}
-    (hg₂ : DPrimrec g₂) :
-    DPrimrec (new% fun x => f_base (g₁_base x) (g₂_base x)) :=
+    {β : Sort v} {β_extra : new_type% β}
+    {γ : β → Sort w} {γ_extra : new_type% γ}
+    {δ : (a : β) → γ a → Sort w'} {δ_extra : new_type% δ}
+    {f : (a : β) → (b : γ a) → δ a b} {f_extra : new_type% f}
+    (hf : DPrimrec (new% fun x : (a : β) ×' γ a => f x.1 x.2))
+    {α : Sort u} {α_extra : new_type% α}
+    {g₁ : α → β} {g₁_extra : new_type% g₁}
+    (hg₁ : DPrimrec g₁_extra)
+    {g₂ : (a : α) → γ (g₁ a)} {g₂_extra : new_type% g₂}
+    (hg₂ : DPrimrec g₂_extra) :
+    DPrimrec (new% fun x => f (g₁ x) (g₂ x)) :=
   .comp hf (New.PSigma.mk.primrec hg₁ hg₂)
 
 protected theorem DComputable.curry
-    {α_base : Sort u} {α : new_type% α_base}
-    {β_base : α_base → Sort v} {β : new_type% β_base}
-    {γ_base : (a : α_base) → β_base a → Sort w} {γ : new_type% γ_base}
-    {f_base : (a : α_base) → (b : β_base a) → γ_base a b} {f : new_type% f_base}
-    (hf : DComputable (new% (fun x : (a : α_base) ×' β_base a => f_base x.1 x.2))) :
-    DComputable (new% f_base) :=
+    {α : Sort u} {α_extra : new_type% α}
+    {β : α → Sort v} {β_extra : new_type% β}
+    {γ : (a : α) → β a → Sort w} {γ_extra : new_type% γ}
+    {f : (a : α) → (b : β a) → γ a b} {f_extra : new_type% f}
+    (hf : DComputable (new% (fun x : (a : α) ×' β a => f x.1 x.2))) :
+    DComputable (new% f) :=
   .of_prim (.curry hf)
 
 protected theorem DComputable.app
-    {ctx_base : Sort u} {ctx : new_type% ctx_base}
-    {α_base : ctx_base → Sort v} {α : new_type% α_base}
-    {β_base : (c : ctx_base) → α_base c → Sort w} {β : new_type% β_base}
-    {f_base : (c : ctx_base) → (a : α_base c) → β_base c a} {f : new_type% f_base}
-    {g_base : (c : ctx_base) → α_base c} {g : new_type% g_base}
-    (hf : DComputable (new% f_base)) (hg : DComputable (new% g_base)) :
-    DComputable (new% fun c => f_base c (g_base c)) := by
+    {ctx : Sort u} {ctx_extra : new_type% ctx}
+    {α : ctx → Sort v} {α_extra : new_type% α}
+    {β : (c : ctx) → α c → Sort w} {β_extra : new_type% β}
+    {f : (c : ctx) → (a : α c) → β c a} {f_extra : new_type% f}
+    {g : (c : ctx) → α c} {g_extra : new_type% g}
+    (hf : DComputable (new% f)) (hg : DComputable (new% g)) :
+    DComputable (new% fun c => f c (g c)) := by
   by_cases hprop : IsProp.{imax v w}
   · exact .of_isProp @(isProp_of_isProp_imax.{v, w} hprop)
   obtain ⟨gf, hgf, hgf'⟩ := hf
@@ -920,7 +923,7 @@ protected theorem DComputable.app
   · rw [← Partrec.nat_iff] at hgf hgg ⊢
     refine .bind hgf (.bind (.comp hgg .fst) (Nat.Partrec.Code.eval_part.comp ?_ .snd))
     exact .comp (.ofNat _) (.comp .snd .fst)
-  · intro a_base a n han
+  · intro a a n han
     obtain ⟨x, hx, hc⟩ := hgf' han
     rw [encoding_pi_def hprop] at hc
     obtain ⟨y, hy, hy'⟩ := hgg' han
@@ -929,16 +932,16 @@ protected theorem DComputable.app
     exact ⟨z, ⟨_, hx, y, hy, by simpa using hz⟩, hz'⟩
 
 theorem dcomputable_curry
-    {α_base : Sort u} {α : new_type% α_base}
-    {β_base : α_base → Sort v} {β : new_type% β_base}
-    {γ_base : (a : α_base) → β_base a → Sort w} {γ : new_type% γ_base}
-    {f_base : (a : α_base) → (b : β_base a) → γ_base a b} {f : new_type% f_base} :
-    DComputable (new% f_base) ↔
-      DComputable (new% fun x : (a : α_base) ×' β_base a => f_base x.1 x.2) := by
+    {α : Sort u} {α_extra : new_type% α}
+    {β : α → Sort v} {β_extra : new_type% β}
+    {γ : (a : α) → β a → Sort w} {γ_extra : new_type% γ}
+    {f : (a : α) → (b : β a) → γ a b} {f_extra : new_type% f} :
+    DComputable (new% f) ↔
+      DComputable (new% fun x : (a : α) ×' β a => f x.1 x.2) := by
   constructor
   · intro f_comp
     refine .app ?_ ?_
-    · refine .app (f := new% fun _ : (a : α_base) ×' β_base a => f_base) ?_ ?_
+    · refine .app (f_extra := new% fun _ : (a : α) ×' β a => f) ?_ ?_
       · exact .constCurry f_comp
       · refine .of_prim ?_
         apply New.PSigma.fst.primrec
