DependentComputability/Tactic/Computability.lean
@@ -57,25 +57,25 @@ attribute [other_dprim] PSigma.fst.dcomp PSigma.snd.dcomp PSigma.mk.dcomp
   PSigma.fst.dprim PSigma.snd.dprim PSigma.mk.dprim
 
 @[dprim]
-theorem _root_.New.Subtype.val.computable.{c, u} {ctx_base : Sort c} {ctx : new_type% ctx_base}
-    {α_base : ctx_base → Sort u} {α : new_type% α_base}
-    {p_base : (c : ctx_base) → α_base c → Prop} {p : new_type% p_base}
-    {self_base : (c : ctx_base) → Subtype (p_base c)} {self : new_type% self_base}
-    (self_comp : DComputable (new% self_base)) :
-    DComputable (new% fun c => (self_base c).val) := by
+theorem _root_.New.Subtype.val.computable.{c, u} {ctx : Sort c} {ctx_extra : new_type% ctx}
+    {α : ctx → Sort u} {α_extra : new_type% α}
+    {p : (c : ctx) → α c → Prop} {p_extra : new_type% p}
+    {self : (c : ctx) → Subtype (p c)} {self_extra : new_type% self}
+    (self_comp : DComputable (new% self)) :
+    DComputable (new% fun c => (self c).val) := by
   obtain ⟨g, hg, hg'⟩ := self_comp
   use g, hg
   simpa using hg'
 
 @[dprim]
-theorem _root_.New.Subtype.mk.computable.{c, u} {ctx_base : Sort c} {ctx : new_type% ctx_base}
-    {α_base : ctx_base → Sort u} {α : new_type% α_base}
-    {p_base : (c : ctx_base) → α_base c → Prop} {p : new_type% p_base}
-    {val_base : (c : ctx_base) → α_base c} {val : new_type% val_base}
-    (val_comp : DComputable (new% val_base))
-    {property_base : (c : ctx_base) → p_base c (val_base c)}
-    (property : new_type% property_base) :
-    DComputable (new% fun c => Subtype.mk (val_base c) (property_base c)) := by
+theorem _root_.New.Subtype.mk.computable.{c, u} {ctx : Sort c} {ctx_extra : new_type% ctx}
+    {α : ctx → Sort u} {α_extra : new_type% α}
+    {p : (c : ctx) → α c → Prop} {p_extra : new_type% p}
+    {val : (c : ctx) → α c} {val_extra : new_type% val}
+    (val_comp : DComputable (new% val))
+    {property : (c : ctx) → p c (val c)}
+    (property_extra : new_type% property) :
+    DComputable (new% fun c => Subtype.mk (val c) (property c)) := by
   obtain ⟨g, hg, hg'⟩ := val_comp
   use g, hg
   simpa using hg'
@@ -120,74 +120,76 @@ convert_to_new Subtype.property
 open Nat.Partrec Denumerable in
 open Lean Elab Tactic in
 theorem _root_.New.Acc.rec.computable.{c, v, u}
-    {ctx_base : Sort c}
-    {ctx : new_type% ctx_base}
-    {α_base : ctx_base → Sort u}
-    {α : new_type% α_base}
-    {r_base : (c : ctx_base) → α_base c → α_base c → Prop}
-    {r : new_type% r_base}
-    {motive_base : (c : ctx_base) → (a : α_base c) → Acc (r_base c) a → Sort v}
-    {motive : new_type% motive_base}
-    {intro_base : (c : ctx_base) → (a : α_base c) →
-        (h : ∀ b, r_base c b a → Acc (r_base c) b) →
-      (ih : ∀ b hb, motive_base c b (h b hb)) → motive_base c a (Acc.intro a h)}
-    {intro : new_type% intro_base}
-    (intro_comp : DComputable (new% intro_base))
-    {a_base : (c : ctx_base) → α_base c}
-    {a : new_type% a_base}
-    (a_comp : DComputable (new% a_base))
-    {t_base : (c : ctx_base) → Acc (r_base c) (a_base c)}
-    {t : new_type% t_base} :
+    {ctx : Sort c}
+    {ctx_extra : new_type% ctx}
+    {α : ctx → Sort u}
+    {α_extra : new_type% α}
+    {r : (c : ctx) → α c → α c → Prop}
+    {r_extra : new_type% r}
+    {motive : (c : ctx) → (a : α c) → Acc (r c) a → Sort v}
+    {motive_extra : new_type% motive}
+    {intro : (c : ctx) → (a : α c) →
+        (h : ∀ b, r c b a → Acc (r c) b) →
+      (ih : ∀ b hb, motive c b (h b hb)) → motive c a (Acc.intro a h)}
+    {intro_extra : new_type% intro}
+    (intro_comp : DComputable (new% intro))
+    {a : (c : ctx) → α c}
+    {a_extra : new_type% a}
+    (a_comp : DComputable (new% a))
+    {t : (c : ctx) → Acc (r c) (a c)}
+    {t_extra : new_type% t} :
     DComputable (new% fun c => @Acc.rec
-      (α_base c) (r_base c) (motive_base c) (intro_base c) (a_base c) (t_base c)) := by
+      (α c) (r c) (motive c) (intro c) (a c) (t c)) := by
   by_cases hprop : IsProp.{imax (max (max 1 u) (imax (max 1 u) v)) v}
   · exact .of_isProp @(isProp_of_isProp_imax.{max (max 1 u) (imax (max 1 u) v), v} hprop)
   by_cases hprop : IsProp.{imax (max 1 u) v}
   · exact .of_isProp @(isProp_of_isProp_imax.{max 1 u, v} hprop)
-  have_new this' : DComp (fun (c : ctx_base)
-      (f : (a : α_base c) → (h : ∀ b, r_base c b a → Acc (r_base c) b) →
-      (ih : ∀ b hb, motive_base c b (h b hb)) → motive_base c a (Acc.intro a h)) =>
-        fun a : (a : { a : α_base c // ∀ b, r_base c b a → Acc (r_base c) b }) ×'
-          ((b : { b : α_base c // r_base c b a }) → motive_base c b (a.2 b b.2)) =>
+  have_new this' : DComp (fun (c : ctx)
+      (f : (a : α c) → (h : ∀ b, r c b a → Acc (r c) b) →
+      (ih : ∀ b hb, motive c b (h b hb)) → motive c a (Acc.intro a h)) =>
+        fun a : (a : { a : α c // ∀ b, r c b a → Acc (r c) b }) ×'
+          ((b : { b : α c // r c b a }) → motive c b (a.2 b b.2)) =>
             f a.1 a.1.2 fun b hb => a.2 ⟨b, hb⟩) := by
     other_dcomp_tac
-  have intro_dcomp_base : DComp intro_base := .unsafeIntro
-  have intro_dcomp : new_type% intro_dcomp_base := intro_comp
-  have_new := this'_base.app intro_dcomp_base
-  clear this' this'_base
-  obtain ⟨gi, hgi, hgi'⟩ := this
+  have intro_dcomp : DComp intro := .unsafeIntro
+  have intro_dcomp_extra : new_type% intro_dcomp := intro_comp
+  have_new := this'.app intro_dcomp
+  clear this' this'_extra
+  obtain ⟨gi, hgi, hgi'⟩ := this_extra
   obtain ⟨ga, hga, hga'⟩ := a_comp
   obtain ⟨scw, hscw⟩ := Code.exists_code.mp selfCallWith_part
   obtain ⟨th, hth⟩ := Code.exists_code.mp (thing_part scw)
   have hyc := ycomb_part th
   refine ⟨_, .comp hyc (.pair hgi hga), ?_⟩
-  intro b_base b n hn
+  intro b b_extra n hn
   obtain ⟨na, hna, hna'⟩ := hga' hn
   obtain ⟨ni, hni, hc⟩ := hgi' hn
   let c := Denumerable.ofNat Code ni
   rw [encoding_pi_def ‹_›] at hc
-  clear hga' hgi' intro_comp intro_dcomp intro_dcomp_base this_base
+  clear hga' hgi' intro_comp intro_dcomp intro_dcomp_extra this
   revert hna' hc
   run_tac
     let names : Array Lean.Name := #[`t, `a, `intro, `motive, `r, `α]
-    let b_base := mkIdent `b_base
     let b := mkIdent `b
+    let eb := mkIdent `b_extra
     for nm in names do
       let id := mkIdent nm
-      let bid := mkIdent (nm.appendAfter "_base")
+      let eid := mkIdent (nm.appendAfter "_extra")
       let pid := mkIdent (nm.appendAfter "'")
-      let pbid := mkIdent (nm.appendAfter "_base'")
-      evalTactic (← `(tactic| let +generalize $pid : new_type% $bid $b_base := $id $b))
+      let peid := mkIdent (nm.appendAfter "_extra'")
+      evalTactic (← `(tactic| let +generalize $peid : new_type% $id $b := $eid $eb))
+      evalTactic (← `(tactic| revert $peid))
+      evalTactic (← `(tactic| let +generalize $pid := $id $b))
       evalTactic (← `(tactic| revert $pid))
-      evalTactic (← `(tactic| let +generalize $pbid := $bid $b_base))
-      evalTactic (← `(tactic| revert $pbid))
-  intro α_base' α' r_base' r' motive_base' motive' intro_base' intro' a_base' a' t_base' t' hna' hc
-  clear_value α_base' α' r_base' r' motive_base' motive' intro_base' intro' a_base' a' t_base' t'
-  clear α_base α r_base r motive_base motive intro_base intro a_base a t_base t
+  intro α' α_extra' r' r_extra' motive' motive_extra' intro' intro_extra'
+    a' a_extra' t' t_extra' hna' hc
+  clear_value α' α_extra' r' r_extra' motive' motive_extra'
+    intro' intro_extra' a' a_extra' t' t_extra'
+  clear α α_extra r r_extra motive motive_extra intro intro_extra a a_extra t t_extra
   simp only [Part.eq_some_iff.mpr hni, Part.map_eq_map, Part.map_some, Part.eq_some_iff.mpr hna,
     seq_eq_bind_map, Part.bind_eq_bind, Part.bind_some]
   clear hna hni
-  induction t' generalizing na with | @intro a_base a ha_base ha ih
+  induction t_extra' generalizing na with | @intro a a_extra ha ha_extra ih
   have hycomb : ∃ g, (∀ n, (ofNat Code g).eval n = ycomb th (Nat.pair ni n)) ∧
       ycomb th (Nat.pair ni na) = c.eval (Nat.pair na g) := by
     refine ⟨Encodable.encode (scw.curry (Encodable.encode (th.curry ni))), ?_, ?_⟩
@@ -195,13 +197,14 @@ theorem _root_.New.Acc.rec.computable.{c, v, u}
       simp [hscw, selfCallWith, ycomb]
     · simp [ycomb, hth, thing, c]
   obtain ⟨g, hg, hg'⟩ := hycomb
-  specialize @hc ⟨⟨a_base, ha_base⟩,
-    fun q => @Acc.rec α_base' r_base' motive_base' intro_base' q.1 (ha_base q.1 q.2)⟩
-    ⟨⟨a, @ha⟩, fun _ q => New.Acc.rec α' r' motive' intro' q.1 (ha q.1 q.2)⟩ (Nat.pair na g)
+  specialize @hc ⟨⟨a, ha⟩,
+    fun q => @Acc.rec α' r' motive' intro' q.1 (ha q.1 q.2)⟩
+    ⟨⟨a_extra, @ha_extra⟩, fun _ q =>
+      New.Acc.rec α_extra' r_extra' motive_extra' intro_extra' q.1 (ha_extra q.1 q.2)⟩
+      (Nat.pair na g)
     ⟨by simpa using hna', ?_⟩
-  · simp only [Nat.unpair_pair]
-    rw [encoding_pi_def ‹_›]
-    intro ⟨y_base, hy_base⟩ ⟨y, hy⟩ x h
+  · rw [encoding_pi_def ‹_›]
+    intro ⟨y, hy⟩ ⟨y, hy⟩ x h
     obtain ⟨z, hz, hz'⟩ := ih y hy x h.1
     simp only [hg]
     use z, hz, hz'
@@ -224,9 +227,9 @@ lemma New.Acc.rec.dcomp.{c, v, u} : new_type% @Acc.rec.dcomp.{c, v, u} :=
   fun _ _ _ _ _ _ _ _ _ _ _ hi _ _ _ ha _ _ => New.Acc.rec.computable hi ha
 
 @[dprim]
-theorem New.PUnit.unit.computable.{u, v} {ctx_base : Sort u} {ctx : new_type% ctx_base} :
-    DComputable (new% fun _ : ctx_base => PUnit.unit.{v}) := by
-  refine .const' (x := new% PUnit.unit.{v}) ?_
+theorem New.PUnit.unit.computable.{u, v} {ctx : Sort u} {ctx_extra : new_type% ctx} :
+    DComputable (new% fun _ : ctx => PUnit.unit.{v}) := by
+  refine .const' (x_extra := new% PUnit.unit.{v}) ?_
   exact ⟨0, .zero⟩
 
 @[other_dprim] lemma PUnit.unit.dcomp.{u, v} {ctx : Sort u} :
@@ -246,18 +249,18 @@ example : DComputable (new% fun (x : Nat → (_ : Nat) ×' Nat) y => x (x y).2) 
   dcomp_tac
 
 @[dprim]
-theorem _root_.New.Nat.zero.computable {ctx_base : Sort u} {ctx : new_type% ctx_base} :
-    DComputable (new% fun _ : ctx_base => Nat.zero) := .const' (x := new% Nat.zero) ⟨0, rfl⟩
+theorem _root_.New.Nat.zero.computable {ctx : Sort u} {ctx_extra : new_type% ctx} :
+    DComputable (new% fun _ : ctx => Nat.zero) := .const' (x_extra := new% Nat.zero) ⟨0, rfl⟩
 
 @[other_dprim] lemma Nat.zero.dcomp {ctx : Sort u} : DComp (fun _ : ctx => Nat.zero) := .unsafeIntro
 lemma New.Nat.zero.dcomp : new_type% @Nat.zero.dcomp.{u} := @New.Nat.zero.computable
 
 @[dprim]
-theorem _root_.New.Nat.succ.computable {ctx_base : Sort u} {ctx : new_type% ctx_base}
-    {f_base : ctx_base → ℕ} {f : new_type% f_base}
-    (f_comp : DComputable (new% f_base)) :
-    DComputable (new% fun c => Nat.succ (f_base c)) := by
-  refine .comp ?_ (f := new% Nat.succ) f_comp
+theorem _root_.New.Nat.succ.computable {ctx : Sort u} {ctx_extra : new_type% ctx}
+    {f : ctx → ℕ} {f_extra : new_type% f}
+    (f_comp : DComputable (new% f)) :
+    DComputable (new% fun c => Nat.succ (f c)) := by
+  refine .comp ?_ (f_extra := new% Nat.succ) f_comp
   refine ⟨Nat.succ, .succ, ?_⟩
   intro a _ _ rfl
   exact ⟨a + 1, by simp, by rfl⟩
@@ -269,33 +272,34 @@ lemma New.Nat.succ.dcomp : new_type% @Nat.succ.dcomp.{u} :=
   fun _ _ _ _ _ hf => New.Nat.succ.computable hf
 
 @[dprim]
-theorem _root_.New.Nat.rec.primrec {ctx_base : Sort u} {ctx : new_type% ctx_base}
-    {motive_base : ctx_base → ℕ → Sort v} {motive : new_type% motive_base}
-    {zero_base : (c : ctx_base) → motive_base c .zero}
-    {zero : new_type% zero_base}
-    (zero_comp : DPrimrec (new% zero_base))
-    {succ_base : (c : ctx_base) → (n : ℕ) → motive_base c n → motive_base c (.succ n)}
-    {succ : new_type% succ_base}
+theorem _root_.New.Nat.rec.primrec {ctx : Sort u} {ctx_extra : new_type% ctx}
+    {motive : ctx → ℕ → Sort v} {motive_extra : new_type% motive}
+    {zero : (c : ctx) → motive c .zero}
+    {zero_extra : new_type% zero}
+    (zero_comp : DPrimrec (new% zero))
+    {succ : (c : ctx) → (n : ℕ) → motive c n → motive c (.succ n)}
+    {succ_extra : new_type% succ}
     (succ_comp : DPrimrec (new%
-      fun x : (c : ctx_base) ×' (n : ℕ) ×' motive_base c n => succ_base x.1 x.2.1 x.2.2))
-    {t_base : ctx_base → ℕ} {t : new_type% t_base}
-    (t_comp : DPrimrec (new% t_base)) :
+      fun x : (c : ctx) ×' (n : ℕ) ×' motive c n => succ x.1 x.2.1 x.2.2))
+    {t : ctx → ℕ} {t_extra : new_type% t}
+    (t_comp : DPrimrec (new% t)) :
     DPrimrec (new% fun c =>
-      @Nat.rec (motive_base c) (zero_base c) (succ_base c) (t_base c)) := by
+      @Nat.rec (motive c) (zero c) (succ c) (t c)) := by
   obtain ⟨fz, hfz, hfz'⟩ := zero_comp
   obtain ⟨fs, hfs, hfs'⟩ := succ_comp
   obtain ⟨ft, hft, hft'⟩ := t_comp
   refine ⟨_, .comp (.prec hfz hfs) (.pair .id hft), ?_⟩
-  intro c_base c nc hnc
+  intro c c_extra nc hnc
   simp only [Nat.unpaired, id_eq, Nat.unpair_pair]
   specialize hfz' hnc
   specialize hft' hnc
-  rw [show t_base c_base = ft nc from hft']
+  rw [show t c = ft nc from hft']
   induction ft nc with
   | zero => exact hfz'
   | succ k ih =>
-    specialize @hfs' ⟨c_base, k, Nat.rec (zero_base c_base) (succ_base c_base) k⟩
-    specialize @hfs' ⟨c, (), New.Nat.rec (motive c) (zero c) (succ c) ()⟩
+    specialize @hfs' ⟨c, k, Nat.rec (zero c) (succ c) k⟩
+    have : new_type% k := ()
+    specialize @hfs' ⟨c_extra, (), new% Nat.rec (zero c) (succ c) k⟩
     exact @hfs' (Nat.pair nc (Nat.pair k _))
       ⟨by simpa using hnc, by simp; rfl, by simpa using ih⟩
 
@@ -437,163 +441,164 @@ set_option linter.unusedVariables false in
 lemma Nat.pair.dprim {ctx : Sort u} {a : ctx → ℕ} (ha : DPrim a) {b : ctx → ℕ} (hb : DPrim b) :
     DPrim fun c => Nat.pair (a c) (b c) := .unsafeIntro
 
-structure TheoremBuilder.{c} {prectx_base : Sort u} (prectx : new_type% prectx_base) where
-  In (pre_base : prectx_base) (pre : new_type% pre_base) (n : ℕ) : Prop
-  OutPrim (ctx_base : Sort c) (ctx : new_type% ctx_base)
-      (pre_base : ctx_base → prectx_base) (pre : new_type% pre_base) : Prop
-  OutComp (ctx_base : Sort c) (ctx : new_type% ctx_base)
-      (pre_base : ctx_base → prectx_base) (pre : new_type% pre_base) : Prop
-  in_implies_outPrim (ctx_base : Sort c) (ctx : new_type% ctx_base)
-      (pre_base : ctx_base → prectx_base) (pre : new_type% pre_base)
+structure TheoremBuilder.{c} {prectx : Sort u} (prectx_extra : new_type% prectx) where
+  In (pre : prectx) (pre_extra : new_type% pre) (n : ℕ) : Prop
+  OutPrim (ctx : Sort c) (ctx_extra : new_type% ctx)
+      (pre : ctx → prectx) (pre_extra : new_type% pre) : Prop
+  OutComp (ctx : Sort c) (ctx_extra : new_type% ctx)
+      (pre : ctx → prectx) (pre_extra : new_type% pre) : Prop
+  in_implies_outPrim (ctx : Sort c) (ctx_extra : new_type% ctx)
+      (pre : ctx → prectx) (pre_extra : new_type% pre)
       (g : ℕ → ℕ) (hg : Nat.Primrec g)
-      (h : ∀ ⦃c_base c c_n⦄, ctx.2 c c_n → In (pre_base c_base) (pre c) (g c_n)) :
-      OutPrim ctx_base ctx pre_base pre
-  in_implies_outComp (ctx_base : Sort c) (ctx : new_type% ctx_base)
-      (pre_base : ctx_base → prectx_base) (pre : new_type% pre_base)
+      (h : ∀ ⦃c c_extra c_n⦄, ctx_extra.2 c_extra c_n → In (pre c) (pre_extra c_extra) (g c_n)) :
+      OutPrim ctx ctx_extra pre pre_extra
+  in_implies_outComp (ctx : Sort c) (ctx_extra : new_type% ctx)
+      (pre : ctx → prectx) (pre_extra : new_type% pre)
       (g : ℕ →. ℕ) (hg : Nat.Partrec g)
-      (h : ∀ ⦃c_base c c_n⦄, ctx.2 c c_n → ∃ m ∈ g c_n, In (pre_base c_base) (pre c) m) :
-      OutComp ctx_base ctx pre_base pre
+      (h : ∀ ⦃c c_extra c_n⦄, ctx_extra.2 c_extra c_n →
+        ∃ m ∈ g c_n, In (pre c) (pre_extra c_extra) m) :
+      OutComp ctx ctx_extra pre pre_extra
 
 theorem TheoremBuilder.primResult (t : @TheoremBuilder Unit (new% Unit)) (h : t.In _ (new% ()) 0) :
-    ∀ {ctx_base : Sort c} {ctx : new_type% ctx_base},
-      t.OutPrim ctx_base ctx _ (new% fun _ : ctx_base => ()) := by
-  intro ctx_base ctx
-  exact t.in_implies_outPrim ctx_base ctx _ _ _ .zero fun _ _ _ _ => h
+    ∀ {ctx : Sort c} {ctx_extra : new_type% ctx},
+      t.OutPrim ctx ctx_extra _ (new% fun _ : ctx => ()) := by
+  intro ctx ctx_extra
+  exact t.in_implies_outPrim ctx ctx_extra _ _ _ .zero fun _ _ _ _ => h
 
 theorem TheoremBuilder.compResult (t : @TheoremBuilder Unit (new% Unit)) (h : t.In _ (new% ()) 0) :
-    ∀ {ctx_base : Sort c} {ctx : new_type% ctx_base},
-      t.OutComp ctx_base ctx _ (new% fun _ : ctx_base => ()) := by
-  intro ctx_base ctx
-  exact t.in_implies_outComp ctx_base ctx _ _ _ .zero fun _ _ _ _ => ⟨0, ⟨⟨⟩, rfl⟩, h⟩
+    ∀ {ctx : Sort c} {ctx_extra : new_type% ctx},
+      t.OutComp ctx ctx_extra _ (new% fun _ : ctx => ()) := by
+  intro ctx ctx_extra
+  exact t.in_implies_outComp ctx ctx_extra _ _ _ .zero fun _ _ _ _ => ⟨0, ⟨⟨⟩, rfl⟩, h⟩
 
-def TheoremBuilder.base.{c} {prectx_base : Sort u} {prectx : new_type% prectx_base}
-    {α_base : prectx_base → Sort v} (α : new_type% α_base)
-    {f_base : (c : prectx_base) → α_base c} (f : new_type% f_base) :
-    TheoremBuilder.{c} (new% prectx_base) where
-  In _ pre n := (α pre).2 (f pre) n
-  OutPrim _ _ pre_base _ := DPrimrec (new% fun a => f_base (pre_base a))
-  OutComp _ _ pre_base _ := DComputable (new% fun a => f_base (pre_base a))
+def TheoremBuilder.base.{c} {prectx : Sort u} {prectx_extra : new_type% prectx}
+    {α : prectx → Sort v} (α_extra : new_type% α)
+    {f : (c : prectx) → α c} (f_extra : new_type% f) :
+    TheoremBuilder.{c} (new% prectx) where
+  In _ pre n := (α_extra pre).2 (f_extra pre) n
+  OutPrim _ _ pre _ := DPrimrec (new% fun a => f (pre a))
+  OutComp _ _ pre _ := DComputable (new% fun a => f (pre a))
   in_implies_outPrim _ _ _ _ pre_n prim hin := ⟨pre_n, prim, @hin⟩
   in_implies_outComp _ _ _ _ pre_n comp hin := ⟨pre_n, comp, @hin⟩
 
-def TheoremBuilder.baseTransformed.{c} {prectx_base : Sort u} {prectx : new_type% prectx_base}
-    {α_base : prectx_base → Sort v} (α : new_type% α_base)
-    {f_base : (c : prectx_base) → α_base c} (f : new_type% f_base)
+def TheoremBuilder.baseTransformed.{c} {prectx : Sort u} {prectx_extra : new_type% prectx}
+    {α : prectx → Sort v} (α_extra : new_type% α)
+    {f : (c : prectx) → α c} (f_extra : new_type% f)
     (g : ℕ → ℕ) (hg : Nat.Primrec g) :
-    TheoremBuilder.{c} (new% prectx_base) where
-  In _ pre n := (α pre).2 (f pre) (g n)
-  OutPrim _ _ pre_base _ := DPrimrec (new% fun a => f_base (pre_base a))
-  OutComp _ _ pre_base _ := DComputable (new% fun a => f_base (pre_base a))
+    TheoremBuilder.{c} (new% prectx) where
+  In _ pre n := (α_extra pre).2 (f_extra pre) (g n)
+  OutPrim _ _ pre _ := DPrimrec (new% fun a => f (pre a))
+  OutComp _ _ pre _ := DComputable (new% fun a => f (pre a))
   in_implies_outPrim _ _ _ _ pre_n prim hin := ⟨_, hg.comp prim, hin⟩
   in_implies_outComp _ _ _ _ pre_n comp hin := ⟨_, .comp (.of_primrec hg) comp, by simpa using hin⟩
 
 theorem primrec_pair_right (c : ℕ) : Nat.Primrec (fun n => Nat.pair n c) := .pair .id (.const c)
 
-def TheoremBuilder.prepend.{c} {prectx_base : Sort u} {prectx : new_type% prectx_base}
-    {α_base : prectx_base → Sort v} {α : new_type% α_base}
-    (h : TheoremBuilder.{c} (new% (a : prectx_base) ×' α_base a)) :
-    TheoremBuilder.{c} (new% prectx_base) where
-  In pre_base pre n :=
-    ∀ a_base : α_base pre_base, ∀ a : new_type% a_base, ∀ a_n : ℕ, (α pre).2 a a_n →
-      h.In _ (new% PSigma.mk pre_base a_base) (Nat.pair n a_n)
-  OutPrim ctx_base ctx pre_base _pre :=
-    ∀ a_base : (c : ctx_base) → α_base (pre_base c), ∀ a : new_type% a_base, DPrimrec a →
-      h.OutPrim ctx_base ctx _ (new% fun c : ctx_base => PSigma.mk (pre_base c) (a_base c))
-  OutComp ctx_base ctx pre_base _pre :=
-    ∀ a_base : (c : ctx_base) → α_base (pre_base c), ∀ a : new_type% a_base, DComputable a →
-      h.OutComp ctx_base ctx _ (new% fun c : ctx_base => PSigma.mk (pre_base c) (a_base c))
-  in_implies_outPrim ctx_base ctx pre_base pre pre_n prim hin := by
-    intro a_base a ⟨g, hg, hg'⟩
-    refine h.in_implies_outPrim ctx_base ctx _ _ _ (prim.pair hg) ?_
-    intro c_base c cn hcn
-    exact hin hcn (a_base c_base) (a c) (g cn) (hg' hcn)
-  in_implies_outComp ctx_base ctx pre_base pre pre_n comp hin := by
-    intro a_base a ⟨g, hg, hg'⟩
-    refine h.in_implies_outComp ctx_base ctx _ _ _ (comp.pair hg) ?_
-    intro c_base c cn hcn
+def TheoremBuilder.prepend.{c} {prectx : Sort u} {prectx_extra : new_type% prectx}
+    {α : prectx → Sort v} {α_extra : new_type% α}
+    (h : TheoremBuilder.{c} (new% (a : prectx) ×' α a)) :
+    TheoremBuilder.{c} (new% prectx) where
+  In pre pre_extra n :=
+    ∀ a : α pre, ∀ a_extra : new_type% a, ∀ a_n : ℕ, (α_extra pre_extra).2 a_extra a_n →
+      h.In _ (new% PSigma.mk pre a) (Nat.pair n a_n)
+  OutPrim ctx ctx_extra pre _pre_extra :=
+    ∀ a : (c : ctx) → α (pre c), ∀ a_extra : new_type% a, DPrimrec a_extra →
+      h.OutPrim ctx ctx_extra _ (new% fun c : ctx => PSigma.mk (pre c) (a c))
+  OutComp ctx ctx_extra pre _pre_extra :=
+    ∀ a : (c : ctx) → α (pre c), ∀ a_extra : new_type% a, DComputable a_extra →
+      h.OutComp ctx ctx_extra _ (new% fun c : ctx => PSigma.mk (pre c) (a c))
+  in_implies_outPrim ctx ctx_extra pre pre_extra pre_n prim hin := by
+    intro a a_extra ⟨g, hg, hg'⟩
+    refine h.in_implies_outPrim ctx ctx_extra _ _ _ (prim.pair hg) ?_
+    intro c c_extra cn hcn
+    exact hin hcn (a c) (a_extra c_extra) (g cn) (hg' hcn)
+  in_implies_outComp ctx ctx_extra pre pre_extra pre_n comp hin := by
+    intro a a_extra ⟨g, hg, hg'⟩
+    refine h.in_implies_outComp ctx ctx_extra _ _ _ (comp.pair hg) ?_
+    intro c c_extra cn hcn
     obtain ⟨m, hm, hm'⟩ := hg' hcn
     obtain ⟨k, hk, hk'⟩ := hin hcn
     simpa [Seq.seq, Part.eq_some_iff.mpr hm, Part.eq_some_iff.mpr hk]
-      using hk' (a_base c_base) (a c) m hm'
+      using hk' (a c) (a_extra c_extra) m hm'
 
-def TheoremBuilder.prependIrrelevant.{c} {prectx_base : Sort u} {prectx : new_type% prectx_base}
-    {α_base : prectx_base → Sort v} {α : new_type% α_base}
-    (h : TheoremBuilder.{c} (new% (a : prectx_base) ×' α_base a)) :
-    TheoremBuilder.{c} (new% prectx_base) where
-  In pre_base pre n :=
-    ∀ a_base : α_base pre_base, ∀ a : new_type% a_base,
-      h.In _ (new% PSigma.mk pre_base a_base) n
-  OutPrim ctx_base ctx pre_base _pre :=
-    ∀ a_base : (c : ctx_base) → α_base (pre_base c), ∀ a : new_type% a_base,
-      h.OutPrim ctx_base ctx _ (new% fun c : ctx_base => PSigma.mk (pre_base c) (a_base c))
-  OutComp ctx_base ctx pre_base _pre :=
-    ∀ a_base : (c : ctx_base) → α_base (pre_base c), ∀ a : new_type% a_base,
-      h.OutComp ctx_base ctx _ (new% fun c : ctx_base => PSigma.mk (pre_base c) (a_base c))
-  in_implies_outPrim ctx_base ctx pre_base pre pre_n prim hin := by
-    intro a_base a
-    refine h.in_implies_outPrim ctx_base ctx _ _ _ prim ?_
-    intro c_base c cn hcn
-    exact hin hcn (a_base c_base) (a c)
-  in_implies_outComp ctx_base ctx pre_base pre pre_n comp hin := by
-    intro a_base a
-    apply h.in_implies_outComp ctx_base ctx _ _ _ comp ?_
-    intro c_base c cn hcn
+def TheoremBuilder.prependIrrelevant.{c} {prectx : Sort u} {prectx_extra : new_type% prectx}
+    {α : prectx → Sort v} {α_extra : new_type% α}
+    (h : TheoremBuilder.{c} (new% (a : prectx) ×' α a)) :
+    TheoremBuilder.{c} (new% prectx) where
+  In pre pre_extra n :=
+    ∀ a : α pre, ∀ a_extra : new_type% a,
+      h.In _ (new% PSigma.mk pre a) n
+  OutPrim ctx ctx_extra pre _pre_extra :=
+    ∀ a : (c : ctx) → α (pre c), ∀ a_extra : new_type% a,
+      h.OutPrim ctx ctx_extra _ (new% fun c : ctx => PSigma.mk (pre c) (a c))
+  OutComp ctx ctx_extra pre _pre_extra :=
+    ∀ a : (c : ctx) → α (pre c), ∀ a_extra : new_type% a,
+      h.OutComp ctx ctx_extra _ (new% fun c : ctx => PSigma.mk (pre c) (a c))
+  in_implies_outPrim ctx ctx_extra pre pre_extra pre_n prim hin := by
+    intro a a_extra
+    refine h.in_implies_outPrim ctx ctx_extra _ _ _ prim ?_
+    intro c c_extra cn hcn
+    exact hin hcn (a c) (a_extra c_extra)
+  in_implies_outComp ctx ctx_extra pre pre_extra pre_n comp hin := by
+    intro a a_extra
+    apply h.in_implies_outComp ctx ctx_extra _ _ _ comp ?_
+    intro c c_extra cn hcn
     obtain ⟨k, hk, hk'⟩ := hin hcn
-    exact ⟨k, hk, hk' (a_base c_base) (a c)⟩
+    exact ⟨k, hk, hk' (a c) (a_extra c_extra)⟩
 
-def TheoremBuilder.prependFirst.{c} {prectx_base : Sort u} {prectx : new_type% prectx_base}
-    {α_base : prectx_base → Sort v} {α : new_type% α_base}
-    (h : TheoremBuilder.{c} (new% (a : prectx_base) ×' α_base a)) :
-    TheoremBuilder.{c} (new% prectx_base) where
-  In pre_base pre n :=
-    ∀ a_base : α_base pre_base, ∀ a : new_type% a_base, ∀ a_n : ℕ, (α pre).2 a a_n →
-      h.In _ (new% PSigma.mk pre_base a_base) a_n
-  OutPrim ctx_base ctx pre_base _pre :=
-    ∀ a_base : (c : ctx_base) → α_base (pre_base c), ∀ a : new_type% a_base, DPrimrec a →
-      h.OutPrim ctx_base ctx _ (new% fun c : ctx_base => PSigma.mk (pre_base c) (a_base c))
-  OutComp ctx_base ctx pre_base _pre :=
-    ∀ a_base : (c : ctx_base) → α_base (pre_base c), ∀ a : new_type% a_base, DComputable a →
-      h.OutComp ctx_base ctx _ (new% fun c : ctx_base => PSigma.mk (pre_base c) (a_base c))
-  in_implies_outPrim ctx_base ctx pre_base pre pre_n prim hin := by
-    intro a_base a ⟨g, hg, hg'⟩
-    refine h.in_implies_outPrim ctx_base ctx _ _ _ hg ?_
-    intro c_base c cn hcn
-    exact hin hcn (a_base c_base) (a c) (g cn) (hg' hcn)
-  in_implies_outComp ctx_base ctx pre_base pre pre_n comp hin := by
-    intro a_base a ⟨g, hg, hg'⟩
-    refine h.in_implies_outComp ctx_base ctx _ _ _ hg ?_
-    intro c_base c cn hcn
+def TheoremBuilder.prependFirst.{c} {prectx : Sort u} {prectx_extra : new_type% prectx}
+    {α : prectx → Sort v} {α_extra : new_type% α}
+    (h : TheoremBuilder.{c} (new% (a : prectx) ×' α a)) :
+    TheoremBuilder.{c} (new% prectx) where
+  In pre pre_extra n :=
+    ∀ a : α pre, ∀ a_extra : new_type% a, ∀ a_n : ℕ, (α_extra pre_extra).2 a_extra a_n →
+      h.In _ (new% PSigma.mk pre a) a_n
+  OutPrim ctx ctx_extra pre _pre_extra :=
+    ∀ a : (c : ctx) → α (pre c), ∀ a_extra : new_type% a, DPrimrec a_extra →
+      h.OutPrim ctx ctx_extra _ (new% fun c : ctx => PSigma.mk (pre c) (a c))
+  OutComp ctx ctx_extra pre _pre_extra :=
+    ∀ a : (c : ctx) → α (pre c), ∀ a_extra : new_type% a, DComputable a_extra →
+      h.OutComp ctx ctx_extra _ (new% fun c : ctx => PSigma.mk (pre c) (a c))
+  in_implies_outPrim ctx ctx_extra pre pre pre_n prim hin := by
+    intro a a_extra ⟨g, hg, hg'⟩
+    refine h.in_implies_outPrim ctx ctx_extra _ _ _ hg ?_
+    intro c c_extra cn hcn
+    exact hin hcn (a c) (a_extra c_extra) (g cn) (hg' hcn)
+  in_implies_outComp ctx ctx_extra pre pre_extra pre_n comp hin := by
+    intro a a_extra ⟨g, hg, hg'⟩
+    refine h.in_implies_outComp ctx ctx_extra _ _ _ hg ?_
+    intro c c_extra cn hcn
     obtain ⟨m, hm, hm'⟩ := hg' hcn
     obtain ⟨k, hk, hk'⟩ := hin hcn
     simpa [Seq.seq, Part.eq_some_iff.mpr hm, Part.eq_some_iff.mpr hk]
-      using hk' (a_base c_base) (a c) m hm'
+      using hk' (a c) (a_extra c_extra) m hm'
 
-partial def makeTheoremBuilder {α_base : Q(Sort u)} {α : Q(new_type% $α_base)}
-    {β_base : Q($α_base → Sort v)} {β : Q(new_type% $β_base)}
-    {f_base : Q((a : $α_base) → $β_base a)} (f : Q(new_type% $f_base))
+partial def makeTheoremBuilder {α : Q(Sort u)} {α_extra : Q(new_type% $α)}
+    {β : Q($α → Sort v)} {β_extra : Q(new_type% $β)}
+    {f : Q((a : $α) → $β a)} (f_extra : Q(new_type% $f))
     (g : Q(ℕ → ℕ)) (hg : Q(Nat.Primrec $g)) (hadRelevant : Bool)
-    (remainingParams : Nat) (clvl : Level) : MetaM Q(TheoremBuilder.{clvl} $α) := do
-  let .lam nm_base _ b_base bi_base := id β_base | unreachable!
-  let .forallE nnnn dom_base body_base bbbiii := id b_base |
+    (remainingParams : Nat) (clvl : Level) : MetaM Q(TheoremBuilder.{clvl} $α_extra) := do
+  let .lam _ _ b _ := id β | unreachable!
+  let .forallE nnnn dom body bbbiii := id b |
     if g == q(id) then
-      return q(.base $β $f)
+      return q(.base $β_extra $f_extra)
     else
-      return q(.baseTransformed $β $f $g $hg)
-  let .lam nm _ (.lam nm' ttt b bi') bi := id β | unreachable!
-  let mkApp4 (.const ``New.Forall [w₁, w₂]) _ dom _ body := id b | unreachable!
+      return q(.baseTransformed $β_extra $f_extra $g $hg)
+  let .lam nm _ (.lam nm' ttt b bi) bi' := id β_extra | unreachable!
+  let mkApp4 (.const ``New.Forall [w₁, w₂]) _ dom_extra _ body_extra := id b | unreachable!
   --
-  let newLam (x : Expr) : Expr := .lam nm α_base (.lam nm' ttt x bi) bi'
-  have dom_base_lam : Q($α_base → Sort w₁) := .lam nm_base α_base dom_base bi_base
-  have _dom_lam : Q(new_type% $dom_base_lam) := newLam dom
-  have body_base_lam : Q((a : $α_base) → $dom_base_lam a → Sort w₂) :=
-    .lam nm_base α_base (.lam nnnn dom_base body_base bbbiii) bi_base
-  have _body_lam : Q(new_type% $body_base_lam) := newLam body
+  let newLam (x : Expr) : Expr := .lam nm α (.lam nm' ttt x bi) bi'
+  have dom_lam : Q($α → Sort w₁) := .lam nm α dom bi
+  have _dom_lam : Q(new_type% $dom_lam) := newLam dom_extra
+  have body_lam : Q((a : $α) → $dom_lam a → Sort w₂) :=
+    .lam nm α (.lam nnnn dom body bbbiii) bi
+  have _body_lam : Q(new_type% $body_lam) := newLam body_extra
   have : v =QL imax w₁ w₂ := ⟨⟩
-  have : $β_base =Q fun c => ∀ x : $dom_base_lam c, $body_base_lam c x := ⟨⟩
-  have : $β =Q new% fun c => ∀ x : $dom_base_lam c, $body_base_lam c x := ⟨⟩
+  have : $β =Q fun c => ∀ x : $dom_lam c, $body_lam c x := ⟨⟩
+  have : $β_extra =Q new% fun c => ∀ x : $dom_lam c, $body_lam c x := ⟨⟩
   let isRelevant := remainingParams == 0 && !w₁.isAlwaysZero
-  let res : Q(TheoremBuilder.{clvl} (new% PSigma $dom_base_lam)) ←
-    makeTheoremBuilder q(new% fun x : PSigma $dom_base_lam => $f_base x.1 x.2)
+  let res : Q(TheoremBuilder.{clvl} (new% PSigma $dom_lam)) ←
+    makeTheoremBuilder q(new% fun x : PSigma $dom_lam => $f x.1 x.2)
       q($g) q($hg) (hadRelevant || isRelevant) (remainingParams - 1) clvl
   if isRelevant then
     if hadRelevant then
@@ -609,7 +614,7 @@ def makeCtorEncodingProof (ctor : ConstructorVal) (isStruct : Bool) (levels : Li
   unless isStruct do
     return .const (mkNewInductEncodingName ctor.induct ++ shortName) levels
   forallTelescope ctor.type fun vars _body => do
-  withNonBaseVars vars convertTypeSimpleNew fun newVars _baseMap => do
+  withNewVars vars convertTypeSimpleNew fun newVars Map => do
     let params := vars.take ctor.numParams
     let newParams := newVars.take ctor.numParams
     let allParams := params.interleave newParams
@@ -734,12 +739,17 @@ def proveConstructorComputable (ctorName : Name) : MetaM Unit := do
       MonadCacheT.run <| go true 0 primResult #[ctx] #[ctx, ctx'] ctor.numParams #[] baseMap
       MonadCacheT.run <| go false 0 compResult #[ctx] #[ctx, ctx'] ctor.numParams #[] baseMap
 
-#print New.Nat.Partrec.Code._encoding
+#print Nat.Partrec.Code
 #eval! proveConstructorComputable ``Nat.Partrec.Code.zero
 #eval! proveConstructorComputable ``Nat.Partrec.Code.succ
 #eval! proveConstructorComputable ``Nat.Partrec.Code.left
 #eval! proveConstructorComputable ``Nat.Partrec.Code.right
-#eval! proveConstructorComputable ``Nat.Partrec.Code.prec
 #eval! proveConstructorComputable ``Nat.Partrec.Code.pair
 #eval! proveConstructorComputable ``Nat.Partrec.Code.comp
+#eval! proveConstructorComputable ``Nat.Partrec.Code.prec
 #eval! proveConstructorComputable ``Nat.Partrec.Code.rfind'
+
+#eval! proveConstructorComputable ``Std.DHashMap.Raw.mk
+
+#print New.Std.DHashMap.Internal.AssocList
+#print Std.DHashMap.Raw.mk
