DependentComputability/Tactic/LetNew.lean
@@ -7,23 +7,23 @@ partial def letNewHelper (goalType : Expr) (val : Expr) (baseMap : FVarIdMap Exp
   | .letE nm t v b false =>
     let newType ← conversionStepNew.visit t baseMap
     let newValue ← conversionStepNew.visit v baseMap
-    withLetDecl (nm.appendAfter "_base") t v fun var_base => do
-    withLetDecl nm (mkExtraApp newType var_base) newValue fun var => do
+    withLetDecl nm t v fun var_base => do
+    withLetDecl (nm.appendAfter "_extra") (mkExtraApp newType var_base) newValue fun var => do
       let (res, mvar) ← letNewHelper goalType (b.instantiate1 var_base)
         (baseMap.insert var_base.fvarId! var)
       return (← mkLetFVars #[var_base, var] res, mvar)
   | .letE nm t v b true =>
     let newType ← conversionStepNew.visit t baseMap
     let newValue ← conversionStepNew.visit v baseMap
-    withLocalDeclD (nm.appendAfter "_base") t fun var_base => do
-    withLocalDeclD nm (mkExtraApp newType var_base) fun var => do
+    withLocalDeclD nm t fun var_base => do
+    withLocalDeclD (nm.appendAfter "_extra") (mkExtraApp newType var_base) fun var => do
       let (res, mvar) ← letNewHelper goalType (b.instantiate1 var_base)
         (baseMap.insert var_base.fvarId! var)
       return (mkApp2 (← mkLambdaFVars #[var_base, var] res) v newValue, mvar)
   | .lam nm t b bi =>
     let newType ← conversionStepNew.visit t baseMap
-    withLocalDecl (nm.appendAfter "_base") bi t fun var_base => do
-    withLocalDecl nm bi (mkExtraApp newType var_base) fun var => do
+    withLocalDecl nm bi t fun var_base => do
+    withLocalDecl (nm.appendAfter "_extra") bi (mkExtraApp newType var_base) fun var => do
       let (res, mvar) ← letNewHelper goalType (b.instantiate1 var_base)
         (baseMap.insert var_base.fvarId! var)
       return (← mkLambdaFVars #[var_base, var] res, mvar)
